up to date NimFull example

plugins/vdm2isa/examples/Nim/NimFull.thy
@@ -1,18 +1,19 @@
 (*<*)theory NimFull 
 imports VDMToolkit
         "~~/src/HOL/Library/While_Combinator"
+Smart_Isabelle.Smart_Isabelle "~~/src/HOL/Eisbach/Eisbach"
 begin(*>*)
-section {* Introduction *}
+section \<open> Introduction \<close>
 
-text{* 
+text\<open> 
   This theory file is a manual translation of the corresponding Overture VDM model. 
   You are expected to read this document whilst playing with the theory file
   in Isabelle and Overture. 
-*}
+\<close>
 (*************************************************************************)
-section {* Imports *}
+section \<open> Imports \<close>
 
-text {*
+text \<open>
   \begin{vdmsl}[breaklines=true]
   module NimFull
   imports from IO		 functions  println	renamed println;
@@ -26,22 +27,22 @@ text {*
   contains various auxiliary functions translating VDM sequences into Isabelle lists. The 
   \texttt{While\_Combinator.thy} theory provides a while-like operator for the main game play. 
   Moreover, we are not translating the auxiliary IO functions, which are just for Overture model debugging.
-*}
+\<close>
 
 (*************************************************************************)
-section {* VDM values *}
+section \<open> VDM values \<close>
 
-text {* Values are trivial: we add them as @{term abbreviation}s. Notice that we would need
-  to add invariants here about @{typ \<nat>}.  *}
+text \<open> Values are trivial: we add them as @{term abbreviation}s. Notice that we would need
+  to add invariants here about @{typ \<nat>}.  \<close>
 
-text{*
+text\<open>
 \begin{vdmsl}[breaklines=true]
 values
 
 MAX_PILE: nat1 = 20;
 MAX_MOV: nat1 = 3;
 \end{vdmsl}
-*}
+\<close>
 
 abbreviation 
   MAX_PILE :: VDMNat1 where "MAX_PILE \<equiv> 20"
@@ -58,9 +59,9 @@ definition
 where
   "inv_MAX_MOV \<equiv> inv_VDMNat1 MAX_MOV \<and> MAX_MOV < MAX_PILE"
 
-text {* Remember the implicit invariant, from requirements, that @{term "MAX_MOV < MAX_PILE"},
+text \<open> Remember the implicit invariant, from requirements, that @{term "MAX_MOV < MAX_PILE"},
   otherwise a player could play to loose from the beginning. This was not in the Overture Module
-  because we gave explicit values, which implied this invariant. *}
+  because we gave explicit values, which implied this invariant. \<close>
 (*
 consts
   G_MAX_PILE :: VDMNat
@@ -72,11 +73,11 @@ where
   "inv_G_MAX_PILE \<equiv> nat1 G_MAX_PILE"
 *)
 
-text {*
+text \<open>
   The fixing of values was just for the benefit of animating the model in overture. All that
   we really cared about was the axiom (given) that these constants should be @{typ \<nat>}$_1$, and that 
   move limit cannot be the whole pile. 
-*}
+\<close>
 
 axiomatization 
       G_MAX_PILE :: "VDMNat" 
@@ -86,7 +87,7 @@ where
   and (*<*) n1_MM [simp]: (*>*) "G_MAX_MOV > 0"
   and (*<*) n1_MPMM[simp]: (*>*)"G_MAX_MOV < G_MAX_PILE"
 
-text {* Another important observation is the colour code Isabelle uses for \textbf{known}, 
+text \<open> Another important observation is the colour code Isabelle uses for \textbf{known}, 
   \textcolor{blue}{\textbf{free}} and \textcolor{green}{\textbf{bound}} variables. For example,
   in the predicate
   
@@ -96,15 +97,15 @@ text {* Another important observation is the colour code Isabelle uses for \text
   (\textcolor{blue}{\textbf{blue}}) is free (i.e. externally given),
   and @{term e} (\textcolor{green}{\textbf{green}}) is bound 
   (i.e. defined locally in the context of the universal quantifier).
-  *}
+  \<close>
   
 (*************************************************************************)
-section {* VDM types *}
+section \<open> VDM types \<close>
 
 (*-----------------------------------------------------------------------*)
-subsection {* Player *}
+subsection \<open> Player \<close>
 
-text{*
+text\<open>
 \begin{vdmsl}[breaklines=true]
 types 
 
@@ -112,61 +113,111 @@ types
 -- include it in the game play algorithm instead
 Player = <P1> | <P2> ;
 \end{vdmsl}
-*}
+\<close>
 
-text {* VDM enumerated types can be declared as Isabelle data type constants. All that matters 
-  is that @{term "P1 \<noteq>  P2"} and that those are the only values of type @{term Player}. *}
+text \<open> VDM enumerated types can be declared as Isabelle data type constants. All that matters 
+  is that @{term "P1 \<noteq>  P2"} and that those are the only values of type @{term Player}. \<close>
 
 datatype Player = P1 | P2
 
-(*-----------------------------------------------------------------------*)
-subsection {* Move *}
+definition
+  inv_Player :: "Player \<Rightarrow> \<bool>"
+  where
+  "inv_Player p \<equiv> True"
 
-text{*
+(*-----------------------------------------------------------------------*)
+subsection \<open> Move \<close>
+
+text\<open>
 \begin{vdmsl}[breaklines=true]
 Move = nat1
 inv m == m <= MAX_MOV;
 \end{vdmsl}
-*}
+\<close>
 
-text {* We use @{term type_synonym} for VDM types, where type invariants must be explicitly 
+text \<open> We use @{term type_synonym} for VDM types, where type invariants must be explicitly 
   declared as boolean-valued functions. Note in this case, we also add the invariant about @{typ \<nat>}$_1$,
   which says that @{term "m > (0::nat)"} and is defined in theory \texttt{VDMBasic.thy} 
-  imported through \texttt{VDMSeq.thy}. *}
+  imported through \texttt{VDMSeq.thy}. \<close>
 
 type_synonym Move = "VDMNat1"
 
 definition
-  inv_Move :: "Move \<Rightarrow> \<bool>"
+  inv_Move :: "VDMNat1 \<Rightarrow> \<bool>"
 where
   "inv_Move m \<equiv> inv_VDMNat1 m \<and> m \<le> MAX_MOV"  
 
-(*+++++++++++++++++++++++++++++++++++++++++++++++++++++++++++++++++++++++*)
-subsubsection {* Useful lemmas about $Move$ invariant: *}
+value "inv_Move 3"
+value "inv_Move 5"
 
-text {* 
+text \<open> I label initial versions of specification later found to be problematic
+  through failed proof with a trailing $0$. I keep versions here for the sake of
+  exposition of how mistakes can happen and what to do about them. The difference
+  is that the first version uses a quantifier instead of @{term inv_SeqElems}.
+
+  Unfortunately, that necessarily complicates the underlying explanation. Remember
+  that you are expected to read this document whilst playing with the theory file
+  in Isabelle and Overture. 
+\<close>
+
+type_synonym Moves0 = "Move VDMSeq"
+
+(* nth s i = s ! i (Isabellem, zero based)
+   s $ i = s(i)    (VDM in Isabelle, one based *)
+
+value "([10,11,12,20]::Moves0) ! 1"
+
+value "([10,11,12,20]::Moves0) $ 1"
+
+value "[1,1,2,10]::Moves0"
+
+definition
+  inv_Moves0 :: "Moves0 \<Rightarrow> \<bool>"
+  where
+  "inv_Moves0 m \<equiv> \<forall> i \<in> inds m . inv_Move (m $ i)"
+
+value "inv_Moves0 [1,1,2,1,2,3]"
+
+definition
+  inv_Moves0_new :: "Moves0 \<Rightarrow> \<bool>"
+  where
+  "inv_Moves0_new m \<equiv> inv_SeqElems inv_Move m"
+   (* [1,2,3] \<longrightarrow> inv_Move 1 \<and> inv_Move 2 \<and> inv_Move 3 *)
+
+lemma "inv_Moves0_new s = inv_Moves0 s"
+  unfolding inv_Moves0_new_def inv_Moves0_def 
+  apply (induct s, simp_all)
+  apply (simp add: inv_SeqElems_def)
+  oops
+
+find_theorems "inv_SeqElems _ _" 
+
+(*+++++++++++++++++++++++++++++++++++++++++++++++++++++++++++++++++++++++*)
+subsubsection \<open> Useful lemmas about $Move$ invariant: \<close>
+
+text \<open> 
   Proof steps noted with ``\textsf{--SH}'' were discovered with the automated
  proof tool called \textsf{sledgehammer}. If Isabelle knows ``enough'' information
  about newly defined concepts, it often discovers proofs. Identifying what
  ``enough'' means in context is part of the challenge. 
-*}
+\<close>
 
 lemma l_inv_Move_nat1 : 
   "inv_Move m \<Longrightarrow> 0 < m"
-unfolding inv_Move_def inv_VDMNat1_def by simp --"SH"
+unfolding inv_Move_def inv_VDMNat1_def by simp 
 
-text {*
+text \<open>
   \begin{enumerate}
     \item every move $m$ is @{typ \<nat>}$_1$: 
 
     @{thm[display] l_inv_Move_nat1}
   \end{enumerate}
-*}
+\<close>
 
 (*-----------------------------------------------------------------------*)
-subsection {* @{term sum_elems} function *}
+subsection \<open> @{term sum_elems} function \<close>
 
-text{*
+text\<open>
 Isabelle requires declaration before use, hence to define the @{term inv_Moves} we must have
 previously defined @{term sum_elems}. 
 
@@ -188,9 +239,9 @@ sum_elems_measure: seq of Move -> nat
 sum_elems_measure(s) == len s;
 
 \end{vdmsl}
-*}
+\<close>
 
-text{* The sum of moves is defined recursively on the length of the list. 
+text\<open> The sum of moves is defined recursively on the length of the list. 
 Like in VDM, pattern matching is used. In Isabelle you must define a pattern
 for every @{term datatype} constructor. For lists they are empty and cons as in VDM. 
 We also need to explicitly add the precondition about its type invariant implicitly
@@ -207,7 +258,7 @@ Isabelle does not does not check type invariants and requires declaration before
  When pre/post are not declared in Overture, we need to define them in order to ensure
 types are properly checked. 
 
-*}
+\<close>
 
 declare [[show_types]]
 fun
@@ -217,6 +268,7 @@ where
 | (*<*) sum_elemsI [intro!]: (*>*) "sum_elems (x # xs) = x + (sum_elems xs)"
 (* The funny annotations give explicit names for each equation, and instructs Isabelle tools. 
    The commented bracket tells LaTeX not to typeset this in final PDF. *)
+(* using list.exhaust apply blast+ done *)
 
 (*<*)
 theorem " \<forall> s . inv_SeqElems inv_Move s \<longrightarrow> 
@@ -225,7 +277,7 @@ by (meson inv_VDMNat_def linear not_less not_numeral_le_zero)
 (*>*)
 
 (*+++++++++++++++++++++++++++++++++++++++++++++++++++++++++++++++++++++++*)
-subsubsection {* Useful lemmas  *}
+subsubsection \<open> Useful lemmas  \<close>
 
 (*
 lemma l_sum_elems_nat: "inv_SeqElems0 inv_Move s \<Longrightarrow> 0 \<le> sum_elems s"
@@ -237,8 +289,8 @@ prefer 2
 apply (simp add: elems_def)
 apply simp
 apply (erule_tac x=a in ballE)
-unfolding elems_def apply simp_all --"SH"
-unfolding inv_Move_def inv_VDMNat1_def apply simp_all --"SH"
+unfolding elems_def apply simp_all (* SH *)
+unfolding inv_Move_def inv_VDMNat1_def apply simp_all (* SH *)
 (* let's simplify the proof *)
 oops
 *)
@@ -247,20 +299,18 @@ lemma l_sum_elems_nat:
   "inv_SeqElems inv_Move s \<Longrightarrow> 0 \<le> sum_elems s"
 unfolding inv_SeqElems_def
 apply (induct s, simp_all)
-using l_inv_Move_nat1 by fastforce --"SH"
+using l_inv_Move_nat1 by fastforce (* SH *)
 
 lemma l_sum_elems_nat1: 
   "inv_SeqElems inv_Move s \<Longrightarrow> s \<noteq> [] \<Longrightarrow> 0 < sum_elems s"
   apply (induct s)
   apply simp_all                        (* need a lemma about inv_SeqElems inv_Move (x # xs) *)
-  apply (simp add: l_inv_SeqElems_Cons) (* need a lemma about inv_Move x *)
-  apply (erule conjE)
-  apply (frule l_inv_Move_nat1)         (* need a lemma about sum_elems s \<ge> 0*)
+   (*apply (simp add: l_inv_SeqElems_Cons) need a lemma about inv_Move x *)
   apply (frule l_sum_elems_nat) 
   apply simp                            
-txt {* @{subgoals[display,indent=0]} This finishes the proof but I want 
+txt \<open> @{subgoals[display,indent=0]} This finishes the proof but I want 
   to have it discovered by \textsf{sledgehammer}.
-*}
+\<close>
 oops
 
 lemma l_sum_elems_nat1: 
@@ -280,23 +330,23 @@ qed
 (*by (smt inv_SeqElems_def l_inv_Move_nat1 l_sum_elems_nat list.pred_inject(2) sum_elems.elims)*)
 (*by (metis add.right_neutral add_le_cancel_left inv_SeqElems_def 
     l_sum_elems_nat le_less list.pred_inject(2) 
-    not_less sum_elems.elims) --"SH" 
+    not_less sum_elems.elims) (* SH *) 
   by (smt inv_SeqElems_def l_inv_Move_nat1 l_sum_elems_nat list.pred_inject(2) sum_elems.elims) SLOW *)
 
 lemma l_sum_elems_notempty: 
-  "inv_SeqElems inv_Move s \<Longrightarrow> 0 < sum_elems s \<Longrightarrow> s \<noteq> []" by auto --"SH"
+  "inv_SeqElems inv_Move s \<Longrightarrow> 0 < sum_elems s \<Longrightarrow> s \<noteq> []" by auto (* SH *)
 
-text {*
+text \<open>
   \begin{enumerate}
     \item sum of elements for a sequence of $Move$ is @{typ \<nat>}: @{thm[display] l_sum_elems_nat}
     \item sum of elements for a non empty sequence of $Move$ is @{typ \<nat>}$_1$: @{thm[display] l_sum_elems_nat1}
     \item non-empty sequence when sum of elements is @{typ \<nat>}$_1$: @{thm[display] l_sum_elems_notempty}
   \end{enumerate}
-*}
+\<close>
 (*<*)thm l_sum_elems_nat l_sum_elems_nat1 l_sum_elems_notempty(*>*)
 
 (*+++++++++++++++++++++++++++++++++++++++++++++++++++++++++++++++++++++++*)
-subsubsection {* Specification *}
+subsubsection \<open> Specification \<close>
 
 definition
   pre_sum_elems :: "Move VDMSeq \<Rightarrow> \<bool>"
@@ -308,76 +358,50 @@ definition
   post_sum_elems :: "Move VDMSeq \<Rightarrow> VDMNat \<Rightarrow> \<bool>"
 where
   "post_sum_elems s RESULT \<equiv> 
-      inv_SeqElems inv_Move s \<and> inv_VDMNat RESULT \<and>
-      (s \<noteq> [] \<longleftrightarrow> 0 < RESULT)"
+      pre_sum_elems s \<longrightarrow> 
+      (inv_VDMNat RESULT \<and>
+       (s \<noteq> [] \<longleftrightarrow> RESULT > 0))"
 
 lemma "\<forall> s . pre_sum_elems s \<longrightarrow> (\<exists> r . post_sum_elems s r)" 
-by (metis inv_VDMNat_def le_cases n1_MP not_le post_sum_elems_def pre_sum_elems_def)
+by (metis inv_VDMNat_def le_cases n1_MP not_le post_sum_elems_def)
 
-lemma "\<forall> s . pre_sum_elems s \<longrightarrow> (post_sum_elems s (sum_elems s))"
+lemma PO_sum_elems_obl: "\<forall> s . pre_sum_elems s \<longrightarrow> (post_sum_elems s (sum_elems s))"
 by (metis NimFull.sum_elems0 inv_VDMNat_def l_sum_elems_nat1 le_less less_irrefl post_sum_elems_def pre_sum_elems_def) 
 
-text {* Useful properties about @{term sum_elems} specification. *}
+text \<open> Useful properties about @{term sum_elems} specification. \<close>
 
 lemma l_pre_sum_elems: 
   "inv_SeqElems inv_Move s \<Longrightarrow> 0 < sum_elems s \<longleftrightarrow> s \<noteq> []"
-using l_sum_elems_nat1 by auto --"SH"
+using l_sum_elems_nat1 by auto (* SH *)
   
 lemma l_pre_sum_elems_sat: 
   "pre_sum_elems s \<Longrightarrow> 0 < sum_elems s \<longleftrightarrow> s \<noteq> []"
-unfolding l_sum_elems_nat1 pre_sum_elems_def by (simp add: l_pre_sum_elems) --"SH"
+unfolding l_sum_elems_nat1 pre_sum_elems_def by (simp add: l_pre_sum_elems) (* SH *)
 
-text {* These (trivial) intermediate results help us ensure that @{term sum_elems} 
-  specification is satisfiable by helping Isabelle \textsf{sledgehammer} find proofs *}
+text \<open> These (trivial) intermediate results help us ensure that @{term sum_elems} 
+  specification is satisfiable by helping Isabelle \textsf{sledgehammer} find proofs \<close>
 
 (*+++++++++++++++++++++++++++++++++++++++++++++++++++++++++++++++++++++++*)
-subsubsection {* Example PO: auxiliary function satisfiability *}
+subsubsection \<open> Example PO: auxiliary function satisfiability \<close>
 
-text {*
-  Next, we illustrate the general PO setup for all auxiliary functions. 
-  After the translation is complete, one needs to translate proof obligations to ensure
-  pre/post are satisfiable. The theorem layout depends on whether there is an explicit definition 
- for the auxiliary function, given explicit definitions will determine the existential witness(es). 
- For instance, for an implicitly defined VDM function
+text \<open>
+  Next, we illustrate the general PO setup for @{term sum_elems}. For instance, 
+  the theorem  for the explicitly defined @{term sum_elems} function is:
+  
+  @{term[display] "\<forall> s . inv_SeqElems inv_Move s \<longrightarrow> pre_sum_elems s \<longrightarrow> post_sum_elems s (sum_elems s)"}
 
- \begin{vdmsl}[breaklines=true]
- f(i: T1) r: T2
- pre pre_f(i)
- post post_f(i, r)
- \end{vdmsl}
+  That is, given any valid input value (@{term "inv_SeqElems inv_Move ms"}), if the pre condition holds,
+  so ought to hold the post condition. We use a definition to declare such statements as conjectures 
+  and then try to prove them as theorems.
 
- we need to prove this satisfiability theorem in Isabelle:
-
- @{term[display] "\<forall> i . inv_T1 i \<longrightarrow> pre_f i \<longrightarrow> (\<exists> r . inv_T2 r \<and> post_f i r)"}
-
-  whereas, for an explicitly defined VDM function
-
- \begin{vdmsl}[breaklines=true]
- f: T1 -> T2
- f(i) == expr
- pre pre_f(i)
- post post_f(i, RESULT)
- \end{vdmsl}
-
- we need to prove this satisfiability theorem in Isabelle:
- 
- @{term[display] "\<forall> i . inv_T1 i \<longrightarrow> pre_f i \<longrightarrow> inv_T2 expr \<and> post_f i expr"}
-
- \textcolor{red}{\textbf{Notice that if explicit definitions are given, there is no choice for 
+ \textcolor{red}{\textbf{Notice that if explicit definitions are given, there is no choice for
  witness for the proof obligation!}} That is, the commitment in the model presented by the 
  explicit definition (\textit{e.g.}~@{term expr}) must feature in the proof. This will be
  particularly interesting in the proof below about @{term best_move}, where the general case is provable, whereas
  the one with the initial explicit definition of @{term best_move} is not. 
  \textcolor{red}{\textbf{That is, the specification is feasible for some implementation but not
- the one given by the explicit definition!}}
-  For instance, the theorem  for the explicitly defined @{term sum_elems} function is:
-  
-  @{term[display] "\<forall> s . inv_SeqElems inv_Move s \<longrightarrow> pre_sum_elems s \<longrightarrow> post_sum_elems s (sum_elems s)"}
-  
-  That is, given any valid input value (@{term "inv_SeqElems inv_Move ms"}), if the pre condition holds,
-  so ought to hold the post condition. We use a definition to declare such statements as conjectures 
-  and then try to prove them as theorems.
-*}      
+ the one given by the explicit definition!}}  
+\<close>      
 
 definition
   PO_sum_elems_sat_obl :: "\<bool>"
@@ -394,28 +418,29 @@ where
 lemma PO_sum_elems_sat_exp_obl
 by (metis NimFull.sum_elems0 PO_sum_elems_sat_exp_obl_def inv_VDMNat_def l_pre_sum_elems_sat le_less post_sum_elems_def)
 
-text {* We first prove the goal manually, followed by \textsf{sledgehammer} discovered proofs,
-  given the lemmas created below. *}
+text \<open> We first prove the goal manually, followed by \textsf{sledgehammer} discovered proofs,
+  given the lemmas created below. \<close>
 
 theorem PO_sum_elems_sat_obl
-unfolding PO_sum_elems_sat_obl_def post_sum_elems_def pre_sum_elems_def
-apply (intro allI impI conjI)
-apply (rule_tac x="sum_elems s" in exI, intro conjI, assumption)
-apply (simp add: l_sum_elems_nat inv_VDMNat_def)
-by (simp add: l_pre_sum_elems)
+  unfolding PO_sum_elems_sat_obl_def post_sum_elems_def pre_sum_elems_def
+  apply safe
+  apply (rule_tac x="sum_elems s" in exI)
+  apply safe
+    apply (simp add: l_sum_elems_nat inv_VDMNat_def)
+by (simp add: l_pre_sum_elems)+
 
 theorem PO_sum_elems_sat_obl
 by (metis PO_sum_elems_sat_obl_def inv_VDMNat_def 
-    l_pre_sum_elems_sat leD linear post_sum_elems_def) --"SH"
+    l_pre_sum_elems_sat leD linear post_sum_elems_def) (* SH *)
 
 theorem PO_sum_elems_sat_exp_obl
 by (simp add: PO_sum_elems_sat_exp_obl_def inv_VDMNat_def 
-              l_pre_sum_elems l_sum_elems_nat post_sum_elems_def) --"SH"
+              l_pre_sum_elems l_sum_elems_nat post_sum_elems_def) (* SH *)
 
 (*-----------------------------------------------------------------------*)
-subsection {* Moves *}
+subsection \<open> Moves \<close>
 
-text{*
+text\<open>
 \begin{vdmsl}[breaklines=true]
 Moves = seq of Move
 inv s == 
@@ -425,9 +450,9 @@ inv s ==
 	-- last move is always 1, when moves are present, at the end of the game
 	(sum_elems(s) = MAX_PILE => s(len s) = 1)
 \end{vdmsl}
-*}
+\<close>
 
-text {*
+text \<open>
   Because @{term Moves} depends on @{term sum_elems}, it must be declared after it. Moreover,
   its invariant uses sequence application ($s(len s)$), which will need adjustment (see values example below).
   \textsf{value} and \textsf{lemma} commands can be used to explore the space of options
@@ -437,14 +462,14 @@ text {*
   lists are indexed from $0$, whereas VDM sequences are indexed from $1$. 
   Check  our version of sequence application operator (e.g. in VDM $s(x)$, in 
   Isabelle @{term "applyVDMSeq s x"}), particularly when called outside the bounds of the sequence.
-*}
+\<close>
 
 value "[a,b] ! 0"                       
 value "[a,b] ! 1"
 value "[a,b] ! 2"
 value "[a,b] ! nat (len [a,b])"
 value "[a,b] ! nat (len [a,b] - 1)"
-value "applyVDMSeq [a,b] (len [a,b])"
+value "[a,b] $ (len [a,b])"
 
 type_synonym Moves = "Move VDMSeq"
 
@@ -457,14 +482,14 @@ where
       (let r = sum_elems s in 
         post_sum_elems s r \<and>
         r \<le> MAX_PILE \<and> 
-        (r = MAX_PILE \<longrightarrow> applyVDMSeq s (len s) = 1))"  
+        (r = MAX_PILE \<longrightarrow> s $ (len s) = 1))"  
 
-text {* 
+text \<open> 
    Finally, as the type invariant depends on another function, we need to ensure its dependent function(s) (e.g. @{term sum_elems}) 
   precondition(s) features in it. Sometimes \textsf{value} does not
   work\footnote{Like in Overture, in some circumstances Isabelle does not know how to evaluate expressions}. 
   Then, \textsf{lemma} can be used.  
-*}
+\<close>
 
 value "inv_Move 2"
 value "inv_Moves [2,20]"
@@ -473,12 +498,12 @@ value "inv_SeqElems inv_Move [2,3,2,1]"
 value "inv_SeqElems inv_Move [2,3,4,1]"
 
 (*************************************************************************)
-section {* VDM auxiliary functions *}
+section \<open> VDM auxiliary functions \<close>
 
 (*-----------------------------------------------------------------------*)
-subsection {* @{term who_plays_next} *}
+subsection \<open> @{term who_plays_next} \<close>
 
-text{*
+text\<open>
 \begin{vdmsl}[breaklines=true]
 -- isabelle requires declaration before use!
 isFirst: Player -> bool
@@ -490,23 +515,23 @@ who_plays_next(ms) ==
 	if len ms mod 2 = 0 then <P1> else <P2>
 pre isFirst(<P1>);
 \end{vdmsl}
-*}
+\<close>
 
 definition
   who_plays_next :: "Moves \<Rightarrow> Player"
 where 
-  "who_plays_next ms \<equiv> (if (len ms) mod 2 = 0 then P1 else P2)"
+  "who_plays_next ms \<equiv> (if (len ms) vdmmod 2 = 0 then P1 else P2)"
 
 definition 
   isFirst :: "Player \<Rightarrow> \<bool>"
 where
   "isFirst p \<equiv> p = P1"
 
-text {* Given there is no pre/post for @{term isFirst}, and no type invariants to check, 
-   modelling pre/post is optional. \textcolor{red}{\textbf{Make sure you know when this is okay!}}*}
+text \<open> Given there is no pre/post for @{term isFirst}, and no type invariants to check, 
+   modelling pre/post is optional. \textcolor{red}{\textbf{Make sure you know when this is okay!}}\<close>
 
 (*+++++++++++++++++++++++++++++++++++++++++++++++++++++++++++++++++++++++*)
-subsubsection {* Specification *}
+subsubsection \<open> Specification \<close>
 
 definition
   pre_who_plays_next :: "Moves \<Rightarrow> \<bool>"
@@ -516,10 +541,11 @@ where
 definition
   post_who_plays_next :: "Moves \<Rightarrow> Player \<Rightarrow> \<bool>"
 where
-  "post_who_plays_next ms RESULT \<equiv> inv_Moves ms "
+  "post_who_plays_next ms RESULT \<equiv> 
+      pre_who_plays_next ms \<longrightarrow> inv_Player RESULT "
 
 (*+++++++++++++++++++++++++++++++++++++++++++++++++++++++++++++++++++++++*)
-subsubsection {* Satisfiability PO *}
+subsubsection \<open> Satisfiability PO \<close>
 
 definition
   PO_who_plays_next_sat_obl :: "\<bool>"
@@ -528,7 +554,7 @@ where
       pre_who_plays_next s \<longrightarrow> (\<exists> r . post_who_plays_next s r)"
 
 theorem PO_who_plays_next_sat_obl 
-by (simp add: PO_who_plays_next_sat_obl_def post_who_plays_next_def) --"SH"
+by (simp add: PO_who_plays_next_sat_obl_def post_who_plays_next_def inv_Player_def) (* SH *)
 
 definition
   PO_who_plays_next_sat_exp_obl :: "\<bool>"
@@ -537,23 +563,23 @@ where
       pre_who_plays_next s \<longrightarrow> post_who_plays_next s (who_plays_next s)"
 
 theorem PO_who_plays_next_sat_exp_obl 
-by (simp add: PO_who_plays_next_sat_exp_obl_def post_who_plays_next_def) --"SH"
+by (simp add: PO_who_plays_next_sat_exp_obl_def post_who_plays_next_def inv_Player_def) (* SH *)
 
 (*-----------------------------------------------------------------------*)
-subsection {* @{term fair_play} *}
+subsection \<open> @{term fair_play} \<close>
 
-text{*
+text\<open>
 \begin{vdmsl}[breaklines=true]
 fair_play: Player * Moves -> bool
 fair_play(p, ms) == p = who_plays_next(ms);
 \end{vdmsl}
-*}
+\<close>
 
-text{* Notice that in Isabelle, we get curried definitions 
+text\<open> Notice that in Isabelle, we get curried definitions 
   (e.g.~@{term "fair_play"} is called as 
   @{term "fair_play p ms"}) for VDM functions with multiple 
   parameters. 
-*}
+\<close>
 
 definition
   fair_play :: "Player \<Rightarrow> Moves \<Rightarrow> \<bool>"
@@ -561,7 +587,7 @@ where
   "fair_play p ms \<equiv> p = who_plays_next ms"
 
 (*+++++++++++++++++++++++++++++++++++++++++++++++++++++++++++++++++++++++*)
-subsubsection {* Specification *}
+subsubsection \<open> Specification \<close>
 
 definition
   pre_fair_play :: "Player \<Rightarrow> Moves \<Rightarrow> \<bool>"
@@ -571,11 +597,11 @@ where
 definition
   post_fair_play :: "Player \<Rightarrow> Moves \<Rightarrow> \<bool> \<Rightarrow> \<bool>"
 where
-  "post_fair_play p ms RESULT \<equiv> inv_Moves ms \<and> 
-      pre_who_plays_next ms \<and> post_who_plays_next ms p"
+  "post_fair_play p ms RESULT \<equiv> 
+     pre_fair_play p ms \<longrightarrow>  post_who_plays_next ms p"
 
 (*+++++++++++++++++++++++++++++++++++++++++++++++++++++++++++++++++++++++*)
-subsubsection {* Satisfiability PO *}
+subsubsection \<open> Satisfiability PO \<close>
 
 definition
   PO_fair_play_sat_obl :: "\<bool>"
@@ -584,8 +610,8 @@ where
       pre_fair_play p s \<longrightarrow> (\<exists> r . post_fair_play p s r)"
 
 theorem PO_fair_play_sat_obl 
-using PO_fair_play_sat_obl_def post_fair_play_def 
-      post_who_plays_next_def pre_fair_play_def by auto --"SH"
+  by (simp add: PO_fair_play_sat_obl_def inv_Player_def post_fair_play_def post_who_plays_next_def)
+(* SH *)
 
 definition
   PO_fair_play_sat_exp_obl :: "\<bool>"
@@ -594,18 +620,18 @@ where
       pre_fair_play p s \<longrightarrow> post_fair_play p s (fair_play p s)"
 
 theorem PO_fair_play_sat_exp_obl 
-using PO_fair_play_sat_exp_obl_def post_fair_play_def 
-      post_who_plays_next_def pre_fair_play_def by auto --"SH"
+  by (simp add: PO_fair_play_sat_exp_obl_def inv_Player_def post_fair_play_def post_who_plays_next_def)
+(* SH *)
 
 (*-----------------------------------------------------------------------*)
-subsection {* @{term moves_left} *}
+subsection \<open> @{term moves_left} \<close>
 
-text{*
+text\<open>
 \begin{vdmsl}[breaklines=true]
 moves_left: Moves -> nat
 moves_left(ms) == MAX_PILE - sum_elems(ms);
 \end{vdmsl}
-*}
+\<close>
 
 definition
   moves_left :: "Moves \<Rightarrow> VDMNat"
@@ -619,54 +645,23 @@ value "int ((20::nat) - 30)"
 value "MAX_PILE - 30" (*>*)
 
 (*+++++++++++++++++++++++++++++++++++++++++++++++++++++++++++++++++++++++*)
-subsubsection {* Specification *}
+subsubsection \<open> Specification \<close>
 
 definition
   pre_moves_left :: "Moves \<Rightarrow> \<bool>"
 where
   "pre_moves_left ms \<equiv> inv_Moves ms \<and> pre_sum_elems ms"
   
-text {* I label initial versions of specification later found to be problematic
-  through failed proof with a trailing $0$. I keep versions here for the sake of
-  exposition of how mistakes can happen and what to do about them. The difference
-  is that the first version calls @{term post_sum_elems} with the wrong @{term RESULT}.
-
-  Unfortunately, that necessarily complicates the underlying explanation. Remember
-  that you are expected to read this document whilst playing with the theory file
-  in Isabelle and Overture. 
-*}
-
-definition
-  post_moves_left0 :: "Moves \<Rightarrow> VDMNat \<Rightarrow> \<bool>"
-where
-  "post_moves_left0 ms RESULT \<equiv> 
-    inv_Moves ms \<and> inv_VDMNat RESULT \<and>
-    pre_sum_elems ms \<and> 
-    post_sum_elems ms RESULT"
-
 definition
   post_moves_left :: "Moves \<Rightarrow> VDMNat \<Rightarrow> \<bool>"
 where
   "post_moves_left ms RESULT \<equiv> 
-    inv_Moves ms \<and> inv_VDMNat RESULT \<and>
-    pre_sum_elems ms \<and> 
-    post_sum_elems ms (sum_elems ms)"
-(* MISTAKES:*)
-(*    post_sum_elems ms RESULT" *)
-(*\<and>  RESULT = MAX_PILE - sum_elems ms*)
+    pre_moves_left ms \<longrightarrow> 
+      inv_VDMNat RESULT \<and> 
+      post_sum_elems ms (sum_elems ms)"
 
 (*+++++++++++++++++++++++++++++++++++++++++++++++++++++++++++++++++++++++*)
-subsubsection {* Satisfiability PO *}
-
-definition
-  PO_moves_left_sat_obl0 :: "\<bool>"
-where
-  "PO_moves_left_sat_obl0 \<equiv> \<forall> s . inv_Moves s \<longrightarrow> 
-      pre_moves_left s \<longrightarrow> (\<exists> r . post_moves_left0  s r)"
-
-theorem PO_moves_left_sat_obl0 
-by (meson PO_moves_left_sat_obl0_def inv_Moves_def 
-          post_moves_left0_def post_sum_elems_def) --"SH"
+subsubsection \<open> Satisfiability PO \<close>
 
 definition
   PO_moves_left_sat_obl :: "\<bool>"
@@ -676,7 +671,7 @@ where
 
 theorem PO_moves_left_sat_obl 
 by (meson PO_moves_left_sat_obl_def inv_Moves_def 
-          post_moves_left_def post_sum_elems_def) --"SH"
+          post_moves_left_def post_sum_elems_def) (* SH *)
 
 definition
   PO_moves_left_sat_exp_obl :: "\<bool>"
@@ -685,34 +680,57 @@ where
       pre_moves_left s \<longrightarrow> post_moves_left s (moves_left s)"
 
 theorem PO_moves_left_sat_exp_obl 
-using PO_moves_left_sat_exp_obl_def inv_Moves_def inv_VDMNat_def 
-      moves_left_def post_moves_left_def by fastforce --"SH"
+  unfolding PO_moves_left_sat_exp_obl_def inv_Moves_def inv_VDMNat_def 
+      moves_left_def post_moves_left_def Let_def
+  by simp 
 
 (*-----------------------------------------------------------------------*)
-subsection {* @{term play_move} *}
+subsection \<open> @{term vdmtake} \<close>
+
+text \<open>The function @{term take} has been defined for lists in Isabelle. We use the VDMToolkit vdmtake instead.\<close>
+
+value "vdmtake 2 [A,B]"
+value "take 2 [A,B]"
+
+(*-----------------------------------------------------------------------*)
+subsection \<open> @{term seq_prefix} \<close>
+
+text \<open>The function @{term seq_prefix} has been defined inside VDMToolkit.\<close>
+
+value "[(1::nat),2] \<sqsubseteq> [1,2,3]"
+value "[(1::nat),2] \<sqsubseteq> [1,3,2]"
+
+(*-----------------------------------------------------------------------*)
+subsection \<open> @{term play_move} \<close>
    
-text{*
+text\<open>
 \begin{vdmsl}[breaklines=true]
 play_move: Player * Move * Moves -> Moves
 play_move(p, m, s) == s ^ [m]
 pre 
-	-- cannot play to loose, but at the end
-	moves_left(s) <> 1 => m < moves_left(s)
-	
+	-- x cannot play to loose, but at the end
+	-- x cannot play to loose before the end
+	(moves_left(s) <> 1 => m < moves_left(s))
 	and
-	--there must be something to be played
-	moves_left(s) > 0
-
+  -- must play to loose at the end
+	(moves_left(s) = m => m = 1)
 	and
+  --there must be something to be played
+	--moves_left(s) > m
+	--and
 	-- encodes fairness: if even no moves, then it must be <P1>'s turn
 	fair_play(p, s)
 post 
 	-- you play something = implicitly true by the inv of Move
 	sum_elems(s) < sum_elems(RESULT)
 	and
-	sum_elems(s) + m = sum_elems(RESULT) 
+	sum_elems(s) + m = sum_elems(RESULT)
+	and 
+	not fair_play(p, RESULT)
+	and
+	seq_prefix[Move](s, RESULT)
 \end{vdmsl}
-*}
+\<close>
 
 definition
   play_move :: "Player \<Rightarrow> Move \<Rightarrow> Moves \<Rightarrow> Moves"
@@ -720,7 +738,7 @@ where
   "play_move p m s \<equiv> s @ [m]"
 
 (*+++++++++++++++++++++++++++++++++++++++++++++++++++++++++++++++++++++++*)
-subsubsection {* Specification *}
+subsubsection \<open> Specification \<close>
 
 definition
   pre_play_move0 :: "Player \<Rightarrow> Move \<Rightarrow> Moves \<Rightarrow> \<bool>"
@@ -735,85 +753,96 @@ definition
   pre_play_move :: "Player \<Rightarrow> Move \<Rightarrow> Moves \<Rightarrow> \<bool>"
 where
   "pre_play_move p m s \<equiv> 
-      inv_Move m \<and> inv_Moves s \<and> pre_moves_left s \<and> pre_fair_play p s \<and>
+      inv_Player p \<and> inv_Move m \<and> inv_Moves s \<and> pre_moves_left s \<and> pre_fair_play p s \<and>
       post_fair_play p s (fair_play p s) \<and>
-      fair_play p s \<and>
-      m \<le> moves_left s \<and>
-      (moves_left s = m \<longrightarrow> m = 1)"
-      
+      (moves_left s \<noteq> 1 \<longrightarrow> m < moves_left s) \<and>
+      (moves_left s = m \<longrightarrow> m = 1) \<and>
+      fair_play p s"
+      (* m \<le> moves_left s \<and>*)
+
 definition
   post_play_move :: "Player \<Rightarrow> Move \<Rightarrow> Moves \<Rightarrow> Moves \<Rightarrow> \<bool>"
 where
   "post_play_move p m s RESULT \<equiv> 
-      inv_Move m \<and> inv_Moves s \<and> inv_Moves RESULT \<and> 
-      pre_sum_elems s \<and> pre_sum_elems RESULT \<and>
-      post_sum_elems s (sum_elems s) \<and> post_sum_elems RESULT (sum_elems RESULT) \<and> 
-      sum_elems s < sum_elems RESULT \<and>
-      sum_elems s + m = sum_elems RESULT"
-(* TODO: use a let expression ? *)
+      pre_play_move p m s \<longrightarrow> 
+        inv_Moves RESULT \<and> 
+        pre_sum_elems s \<and> pre_sum_elems RESULT \<and>
+        post_sum_elems s (sum_elems s) \<and> post_sum_elems RESULT (sum_elems RESULT) \<and> 
+        sum_elems s < sum_elems RESULT \<and>
+        sum_elems s + m = sum_elems RESULT \<and>
+        \<not> (fair_play p RESULT) \<and>
+        s \<sqsubseteq> RESULT"
 
 (*+++++++++++++++++++++++++++++++++++++++++++++++++++++++++++++++++++++++*)
-subsubsection {* Satisfiability PO *}
+subsubsection \<open> Satisfiability PO \<close>
 
-text {* This PO is rather involved and will be discussed later in the text. *}
+text \<open> This PO is rather involved and will be discussed later in the text. \<close>
 
 (*-----------------------------------------------------------------------*)
-subsection {* @{term will_first_player_win} *}
+subsection \<open> @{term will_first_player_win} \<close>
 
-text{*
+text\<open>
 \begin{vdmsl}[breaklines=true]
 will_first_player_win: () -> bool
 will_first_player_win() == (MAX_PILE - 1) mod (MAX_MOV + 1) <> 0;
 \end{vdmsl}
-*}
+\<close>
 
-text{* VDM parameterless functions are just like constants of the result type. Be careful with
+text\<open> VDM parameterless functions are just like constants of the result type. Be careful with
   expressions like @{term "x (-1::int)"} and @{term "x - (1::int)"}:~the former applies the function $x$ to 
   the parameter $-1$, whereas the second applies the subtraction function to two parameters $x$ and $1$.
   Think of negative numbers as a unary function.
-*}
+\<close>
 
 definition 
-  will_first_player_win :: "\<bool>"
+  will_first_player_win :: "Move \<Rightarrow> \<bool>"
 where
-  "will_first_player_win \<equiv> (MAX_PILE - 1) mod (MAX_MOV + 1) \<noteq> 0"
+  "will_first_player_win limit \<equiv> (MAX_PILE - 1) vdmmod (limit + 1) \<noteq> 0"
 
 (*+++++++++++++++++++++++++++++++++++++++++++++++++++++++++++++++++++++++*)
-subsubsection {* Specification *}
+subsubsection \<open> Specification \<close>
 
 definition 
-  pre_will_first_player_win :: "\<bool>"
+  pre_will_first_player_win :: "Move \<Rightarrow> \<bool>"
 where
-  "pre_will_first_player_win \<equiv> inv_MAX_PILE"
+  "pre_will_first_player_win limit \<equiv> inv_MAX_PILE \<and> inv_Move limit \<and> pre_vdm_mod (MAX_PILE - 1) (limit + 1)"
 
-text {* The precondition is needed to avoid applying the modulo operator to negative numbers *}
+text \<open> The precondition is needed to avoid applying the modulo operator to negative numbers \<close>
   
 (*+++++++++++++++++++++++++++++++++++++++++++++++++++++++++++++++++++++++*)
-subsubsection {* Satisfiability PO *}
+subsubsection \<open> Satisfiability PO \<close>
 
 definition
   PO_will_first_player_win_sat_obl :: "\<bool>"
 where
   "PO_will_first_player_win_sat_obl \<equiv> 
-      pre_will_first_player_win \<longrightarrow> (\<exists> r . r)"
+      \<forall> limit . pre_will_first_player_win limit \<longrightarrow> (\<exists> r . r)"
 
 theorem PO_will_first_player_win_sat_obl 
-using PO_will_first_player_win_sat_obl_def by auto --"SH"
+using PO_will_first_player_win_sat_obl_def by auto (* SH *)
 
 definition
   PO_will_first_player_win_sat_exp_obl :: "\<bool>"
 where
   "PO_will_first_player_win_sat_exp_obl \<equiv> 
-      pre_will_first_player_win \<longrightarrow> will_first_player_win"
+      \<forall> limit . pre_will_first_player_win limit \<longrightarrow> will_first_player_win limit"
 
 theorem PO_will_first_player_win_sat_exp_obl 
-using PO_will_first_player_win_sat_exp_obl_def 
-      pre_will_first_player_win_def  will_first_player_win_def by simp --"SH"
+  unfolding  PO_will_first_player_win_sat_exp_obl_def 
+      will_first_player_win_def pre_will_first_player_win_def  will_first_player_win_def 
+      pre_vdm_mod_def inv_Move_def inv_VDMNat1_def inv_MAX_PILE_def
+  apply simp
+  apply (intro allI impI, elim conjE)
+  txt \<open>proof of specific/individual cases is more difficult, paradoxically\<close>
+  apply (case_tac limit, simp_all)
+  apply (case_tac "n=1", simp_all)
+  apply (case_tac "n=2", simp_all)
+  by (case_tac "n=3", simp_all)
 
 (*-----------------------------------------------------------------------*)
-subsection {* @{term who_won_invariant} *}
+subsection \<open> @{term who_won_invariant} \<close>
 
-text {*
+text \<open>
 \begin{vdmsl}[breaklines=true]
 -- invariant for whoever won: last player looses by taking 1
 -- even seq means second player; odd seq means firs player 
@@ -828,74 +857,75 @@ who_won_invariant(winner, moves) ==
 	and
 	will_first_player_win() => isFirst(winner) 
 \end{vdmsl}
-*}
+\<close>
 
 definition
-  who_won_invariant :: "Player \<Rightarrow> Moves \<Rightarrow> \<bool>"
+  who_won_invariant :: "Player \<Rightarrow> Moves \<Rightarrow> Move \<Rightarrow> \<bool>"
 where
-  "who_won_invariant winner moves \<equiv> 
+  "who_won_invariant winner moves limit \<equiv> 
       moves_left moves = 0
       \<and>
       winner = who_plays_next moves
       \<and>
-      will_first_player_win \<longrightarrow> isFirst winner"
+      will_first_player_win limit \<longrightarrow> isFirst winner"
 
 (*+++++++++++++++++++++++++++++++++++++++++++++++++++++++++++++++++++++++*)
-subsubsection {* Specification *}
+subsubsection \<open> Specification \<close>
 
 definition
-  pre_who_won_invariant :: "Player \<Rightarrow> Moves \<Rightarrow> \<bool>"
+  pre_who_won_invariant :: "Player \<Rightarrow> Moves \<Rightarrow> Move \<Rightarrow> \<bool>"
 where
-  "pre_who_won_invariant winner moves \<equiv> 
+  "pre_who_won_invariant winner moves limit \<equiv> 
       inv_Moves moves \<and> pre_moves_left moves \<and> 
-      pre_will_first_player_win \<and> pre_who_plays_next moves" 
+      pre_will_first_player_win limit \<and> pre_who_plays_next moves" 
 
 definition
-  post_who_won_invariant :: "Player \<Rightarrow> Moves \<Rightarrow> \<bool> \<Rightarrow> \<bool>"
+  post_who_won_invariant :: "Player \<Rightarrow> Moves \<Rightarrow> Move \<Rightarrow> \<bool> \<Rightarrow> \<bool>"
 where
-  "post_who_won_invariant winner moves RESULT \<equiv> 
-      inv_Moves moves \<and> pre_moves_left moves \<and> 
+  "post_who_won_invariant winner moves limit RESULT \<equiv> 
+      pre_who_won_invariant winner moves limit \<longrightarrow>
       post_moves_left moves (moves_left moves) \<and>
-      pre_will_first_player_win \<and> 
-      pre_who_plays_next moves \<and> post_who_plays_next moves winner" 
+      post_who_plays_next moves winner" 
 
 (*+++++++++++++++++++++++++++++++++++++++++++++++++++++++++++++++++++++++*)
-subsubsection {* Satisfiability PO *}
+subsubsection \<open> Satisfiability PO \<close>
 
 definition
   PO_who_won_invariant_sat_obl :: "\<bool>"
 where
-  "PO_who_won_invariant_sat_obl \<equiv> \<forall> s p . inv_Moves s \<longrightarrow> 
-      pre_who_won_invariant p s \<longrightarrow> (\<exists> r . post_who_won_invariant p s r)"
+  "PO_who_won_invariant_sat_obl \<equiv> \<forall> s p l . 
+      pre_who_won_invariant p s l \<longrightarrow> (\<exists> r . post_who_won_invariant p s l r)"
 
 theorem PO_who_won_invariant_sat_obl 
 unfolding PO_who_won_invariant_sat_obl_def post_who_won_invariant_def 
      pre_who_won_invariant_def
 using inv_Moves_def inv_VDMNat_def moves_left_def 
-      post_moves_left_def post_who_plays_next_def oops (*by fastforce --"SH"*)
+      post_moves_left_def post_who_plays_next_def oops (*by fastforce (* SH *)*)
 
 definition
   PO_who_won_invariant_sat_exp_obl :: "\<bool>"
 where
-  "PO_who_won_invariant_sat_exp_obl \<equiv> \<forall> s p . inv_Moves s \<longrightarrow> 
-      pre_who_won_invariant p s \<longrightarrow> post_who_won_invariant p s (who_won_invariant p s)"
+  "PO_who_won_invariant_sat_exp_obl \<equiv> \<forall> s p l . 
+      pre_who_won_invariant p s l \<longrightarrow> post_who_won_invariant p s l (who_won_invariant p s l)"
 
 theorem PO_who_won_invariant_sat_exp_obl 
 unfolding PO_who_won_invariant_sat_exp_obl_def post_who_won_invariant_def 
      pre_who_won_invariant_def
 using inv_Moves_def inv_VDMNat_def moves_left_def 
-      post_moves_left_def post_who_plays_next_def oops(*by fastforce --"SH"*)
+      post_moves_left_def post_who_plays_next_def 
+  apply simp 
+  oops
       
 (*-----------------------------------------------------------------------*)
-subsection {*  @{term first_player} *}
+subsection \<open>  @{term first_player} \<close>
 
-text{*
+text\<open>
 \begin{vdmsl}[breaklines=true]
 first_player: () -> Player
 first_player() == if isFirst(<P1>) then <P1> else <P2>
 post isFirst(RESULT);
 \end{vdmsl}
-*}
+\<close>
 
 definition
   first_player :: "Player"
@@ -903,7 +933,7 @@ where
   "first_player \<equiv> (if isFirst P1 then P1 else P2)"
 
 (*+++++++++++++++++++++++++++++++++++++++++++++++++++++++++++++++++++++++*)
-subsubsection {* Specification *}
+subsubsection \<open> Specification \<close>
 
 definition
   post_first_player :: "Player \<Rightarrow> \<bool>"
@@ -911,7 +941,7 @@ where
   "post_first_player RESULT \<equiv> isFirst RESULT" 
 
 (*+++++++++++++++++++++++++++++++++++++++++++++++++++++++++++++++++++++++*)
-subsubsection {* Satisfiability PO *}
+subsubsection \<open> Satisfiability PO \<close>
 
 definition
   PO_first_player_sat_obl :: "\<bool>"
@@ -920,7 +950,7 @@ where
 
 theorem PO_first_player_sat_obl 
 unfolding PO_first_player_sat_obl_def post_first_player_def 
-by (simp add: isFirst_def) --"SH"
+by (simp add: isFirst_def) (* SH *)
 
 definition
   PO_first_player_sat_exp_obl :: "\<bool>"
@@ -930,18 +960,18 @@ where
 theorem PO_first_player_sat_exp_obl 
 unfolding PO_first_player_sat_exp_obl_def post_first_player_def 
      first_player_def
-by (simp add: isFirst_def) --"SH"
+by (simp add: isFirst_def) (* SH *)
   
 (*-----------------------------------------------------------------------*)
-subsection {* @{term first_player_inds} *}
+subsection \<open> @{term first_player_inds} \<close>
 
-text{*
+text\<open>
 \begin{vdmsl}[breaklines=true]
 first_player_inds: Moves -> set of nat1
 first_player_inds(ms) == { i | i in set inds ms & i mod 2 <> 0 }
 post RESULT subset inds ms;
 \end{vdmsl}
-*}
+\<close>
 
 definition
   first_player_inds :: "Moves \<Rightarrow> VDMNat1 VDMSet"
@@ -949,14 +979,14 @@ where
   "first_player_inds ms \<equiv> { i | i . i \<in> inds ms \<and> i mod 2 \<noteq> 0 }"
  (* TODO: explain why we need @{term inds_as_nat} here. *)
 
-text {* 
+text \<open> 
   Again, \textsf{value} and \textsf{lemma} commands can be used to explore the space of 
   options desired. Whenever \textsf{value} fails (see commented expression in theory file), 
   that is because Isabelle does not know
   how to enumerate the expression, like in certain circumstances Overture cannot execute models. 
   For that, we can use lemmas and simple proofs. The ``proof'' here is really debugging as 
   we do not know whether the expected expression means what we want/intend, hence the @{term oops} command.
-*}
+\<close>
 value "{i . i\<in> {(0::int),1,2,3}}"
 value "{(i,i)| i . i\<in> {(0::int),1,2,3} }"
 (*value "{i . i\<in> {(0::int),1,2,3} | i < 2}"*)
@@ -965,7 +995,7 @@ lemma "A = {i | i . i\<in> {(0::int),1,2,3} \<and> i < 2}" apply simp oops
 lemma "{0,1} = {i | i . i\<in> {(0::int),1,2,3} \<and> i < 2}" apply auto done
 
 (*+++++++++++++++++++++++++++++++++++++++++++++++++++++++++++++++++++++++*)
-subsubsection {* Specification *}
+subsubsection \<open> Specification \<close>
 
 definition
   pre_first_player_inds :: "Moves \<Rightarrow> \<bool>"
@@ -979,7 +1009,7 @@ where
       inv_SetElems inv_VDMNat1 RESULT \<and> RESULT \<subseteq> inds ms" 
 
 (*+++++++++++++++++++++++++++++++++++++++++++++++++++++++++++++++++++++++*)
-subsubsection {* Satisfiability PO *}
+subsubsection \<open> Satisfiability PO \<close>
 
 definition
   PO_first_player_inds_sat_obl :: "\<bool>"
@@ -988,7 +1018,7 @@ where
       pre_first_player_inds s \<longrightarrow> (\<exists> r . post_first_player_inds s r)"
 
 theorem PO_first_player_inds_sat_obl 
-using PO_first_player_inds_sat_obl_def inv_SetElems_def post_first_player_inds_def by auto --"SH"
+using PO_first_player_inds_sat_obl_def inv_SetElems_def post_first_player_inds_def by auto (* SH *)
 
 definition
   PO_first_player_inds_sat_exp_obl :: "\<bool>"
@@ -999,7 +1029,8 @@ where
 lemma l_first_player_inds_nat1: 
   "inv_Moves s \<Longrightarrow> inv_SetElems inv_VDMNat1 (first_player_inds s)"
   unfolding first_player_inds_def inds_as_nat_def len_def inv_SetElems_def inv_VDMNat1_def
-  by (simp add: VDMSeq_def(2)) --"SH"
+  unfolding  inds_def
+  by (simp)
 
 lemma l_first_player_inds_within_inds: 
   "first_player_inds s \<subseteq> inds s"
@@ -1016,24 +1047,24 @@ apply (simp add: l_first_player_inds_nat1)
 by (simp add: l_first_player_inds_within_inds)
 
 (*-----------------------------------------------------------------------*)
-subsection {* @{term moves_of} *}
+subsection \<open> @{term moves_of} \<close>
 
-text{*
+text\<open>
 \begin{vdmsl}[breaklines=true]
 moves_of: Moves * bool -> seq of Move
 moves_of(ms, first) == 
 	let idxs = first_player_inds(ms) in
 			[ ms(i) | i in set  if (first) then idxs else inds ms \ idxs ]
 \end{vdmsl}
-*}
+\<close>
 
-text {*
+text \<open>
   Isabelle does not allow for sets to bound variables used in list comprehension generators. 
   That means either you need to use a sequence as a generator, or transform a set into a 
   sorted list (by the ordering of the underlying elements). If the set of elements does not 
   have a defined order sorting will fail. Also, @{term sorted_list_of_set} can lead to 
   complicated proofs. Avoid if possible. I show it here in case you are keen on using it.
-*}
+\<close>
 
 (*value "[ [a,b,c] ! i . i \<leftarrow> inds [a,b,c]]" = doesn't like sets for generators *)
 value "[ [a,b,c] ! i . i \<leftarrow> [2,1,0]]"
@@ -1048,7 +1079,7 @@ where
         [ ms ! (nat i) . i \<leftarrow> sorted_list_of_set (if first then idxs else (inds ms - idxs)) ])"
 
 (*+++++++++++++++++++++++++++++++++++++++++++++++++++++++++++++++++++++++*)
-subsubsection {* Specification *}
+subsubsection \<open> Specification \<close>
 
 definition
   pre_moves_of :: "Moves \<Rightarrow> \<bool> \<Rightarrow> \<bool>"
@@ -1063,13 +1094,13 @@ where
       pre_first_player_inds ms \<and> post_first_player_inds ms (first_player_inds ms)"
 
 (*+++++++++++++++++++++++++++++++++++++++++++++++++++++++++++++++++++++++*)
-subsubsection {* Satisfiability PO *}
+subsubsection \<open> Satisfiability PO \<close>
 
 definition
   PO_moves_of_sat_obl :: "\<bool>"
 where
-  "PO_moves_of_sat_obl \<equiv> \<forall> s f . inv_Moves s \<longrightarrow> 
-      pre_moves_of s f \<longrightarrow> (\<exists> r . post_moves_of s f r)"
+  "PO_moves_of_sat_obl \<equiv> 
+      \<forall> s f . pre_moves_of s f \<longrightarrow> (\<exists> r . post_moves_of s f r)"
 
 theorem PO_moves_of_sat_obl 
 unfolding PO_moves_of_sat_obl_def post_moves_of_def  pre_moves_of_def 
@@ -1097,36 +1128,36 @@ apply simp
 unfolding post_first_player_inds_def pre_first_player_inds_def
 apply simp
 apply (intro allI impI conjI)
-(*apply (simp add: l_moves_of_move) --"SH"*)
+(*apply (simp add: l_moves_of_move) (* SH *)*)
 defer
-apply (simp add: l_first_player_inds_nat1) --"SH"
-apply (simp add: l_first_player_inds_within_inds) --"SH"
+apply (simp add: l_first_player_inds_nat1) (* SH *)
+apply (simp add: l_first_player_inds_within_inds) (* SH *)
 oops
 
 (*-----------------------------------------------------------------------*)
-subsection {* @{term best_move} *}
+subsection \<open> @{term best_move} \<close>
 
-text{*
+text\<open>
 \begin{vdmsl}[breaklines=true]
 best_move: Moves -> nat
 best_move(moves) == (moves_left(moves) - 1) mod (MAX_MOV + 1);
 post RESULT <= moves_left(moves);
 \end{vdmsl}
-*}
+\<close>
 
 definition
   best_move :: "Moves \<Rightarrow> VDMNat"
 where
-  "best_move moves \<equiv> ((moves_left moves) - 1) mod (MAX_MOV + 1)"
+  "best_move moves \<equiv> ((moves_left moves) - 1) vdmmod (MAX_MOV + 1)"
 
 (*+++++++++++++++++++++++++++++++++++++++++++++++++++++++++++++++++++++++*)
-subsubsection {* Specification *}
+subsubsection \<open> Specification \<close>
 
-text {* Here I explore a few versions of the specification, first the 
+text \<open> Here I explore a few versions of the specification, first the 
  original one, which was shown to be mistaken after proofs below.
   The first precondition misses the fact @{term "moves_left ms > 0"},
   which prevents modulo arithmetic over negative numbers, whereas the
-  first post condition used the wrong specification of @{term post_moves_left0}. *}
+  first post condition used the wrong specification of @{term post_moves_left0}. \<close>
 
 definition
   pre_best_move0 :: "Moves \<Rightarrow> \<bool>"
@@ -1138,7 +1169,7 @@ definition
 where
   "post_best_move0 ms RESULT \<equiv> 
       inv_Moves ms \<and> inv_VDMNat RESULT \<and>
-      pre_moves_left ms \<and> post_moves_left0 ms (moves_left ms) \<and>
+      pre_moves_left ms \<and> post_moves_left ms (moves_left ms) \<and>
       RESULT \<le> moves_left ms" 
 
 definition
@@ -1155,9 +1186,9 @@ where
       RESULT \<le> moves_left ms" 
 
 (*+++++++++++++++++++++++++++++++++++++++++++++++++++++++++++++++++++++++*)
-subsubsection {* Satisfiability PO *}
+subsubsection \<open> Satisfiability PO \<close>
 
-text {*
+text \<open>
   After the translation is complete, one needs to create proof obligations to ensure
   pre/post are satisfiable. For instance, the theorem layout for @{term best_move} is:
   
@@ -1173,7 +1204,7 @@ Next we show the various proof attempts for the PO conjecture.
 \begin{enumerate}
   \item[1] Naive attempt:~layered expansion followed by simplification.
 \end{enumerate}
-*}      
+\<close>      
 
 definition
   PO_best_move_sat_obl0 :: "\<bool>"
@@ -1181,94 +1212,105 @@ where
   "PO_best_move_sat_obl0 \<equiv> \<forall> ms . inv_Moves ms \<longrightarrow> 
       pre_best_move0 ms \<longrightarrow> (\<exists> r . post_best_move0 ms r)"
 
-  value "3 +(5::int)"
+value "3 +(5::int)"
+
+lemma l_moves_left_nat: 
+  "inv_Moves ms \<Longrightarrow> 0 \<le> moves_left ms"
+unfolding moves_left_def inv_Moves_def Let_def by simp
+
 theorem PO_best_move_sat_obl0
 unfolding PO_best_move_sat_obl0_def 
            pre_best_move0_def post_best_move0_def
 find_theorems "\<forall> _ . (_ \<longrightarrow> _)"
 apply simp
-unfolding pre_moves_left_def post_moves_left0_def
+unfolding pre_moves_left_def post_moves_left_def
 apply simp
 unfolding pre_sum_elems_def post_sum_elems_def
 apply simp
 unfolding  inv_VDMNat_def 
 apply auto 
 apply (rule_tac x=0 in exI, intro conjI, simp_all)
-txt {* @{subgoals[display,indent=0]} 
+txt \<open> @{subgoals[display,indent=0]} 
 
   Missing cases where we cannot make progress suggest we need lemmas on @{term "0 \<le> moves_left ms"}.
   There is also an error: @{term "moves_left ms = 0"} and yet @{term "ms \<noteq> []"}! 
   We will need to change to @{term "post_moves_left"} from @{term post_moves_left0}.
-*}
+\<close>
+  prefer 2 
+   apply (simp add: l_sum_elems_nat)
+  prefer 2
+  using l_sum_elems_nat1 apply auto[1]
+   apply (simp add: l_moves_left_nat)+
 oops
 
-text {*
+text \<open>
   The simplistic strategy of expanding and simplifying does not work here. We need intermediate 
   results to help Isabelle finish the proof. That means, being creative about adequate auxiliary lemmas.
-*}
-
-lemma l_moves_left_nat: 
-  "inv_Moves ms \<Longrightarrow> 0 \<le> moves_left ms"
-unfolding moves_left_def inv_Moves_def Let_def by simp
+\<close>
 
 lemma l_moves_left_nat1: 
   "inv_Moves ms \<Longrightarrow> 0 < moves_left ms"
 apply (induct ms)
 unfolding moves_left_def
 apply simp_all
-txt {* @{subgoals[display,indent=0]}
+txt \<open> @{subgoals[display,indent=0]}
   Missing lemma about @{term "inv_Moves (x # xs)"} distributing over list append.
-*}
+\<close>
 oops
 
 lemma l_inv_Moves_Cons: 
   "inv_Moves (x # xs) = (inv_Move x \<and> inv_Moves xs)"
 apply (intro iffI conjI)
-txt {* @{subgoals[display,indent=0]}
+txt \<open> @{subgoals[display,indent=0]}
   Let us split the work again into lemmas for each subgoal to help \textsf{sledgehammer}!
-*}
+\<close>
 oops
 
+declare[[show_types=false]]
 lemma l_inv_Moves_Hd: 
   "inv_Moves (x # xs) \<Longrightarrow> inv_Move x"
-unfolding inv_Moves_def by (simp add: l_inv_SeqElems_Cons) --"SH"
+  unfolding inv_Moves_def 
+    by (simp add: l_inv_SeqElems_Cons)
 
 lemma l_inv_Moves_Tl: 
   "inv_Moves (x # xs) \<Longrightarrow> inv_Moves xs"
 unfolding inv_Moves_def
 apply (intro conjI) 
-apply (simp add: l_inv_SeqElems_Cons) --"SH"
-apply (simp add: l_inv_SeqElems_Cons pre_sum_elems_def) --"SH"
+apply (simp) (* SH *)
+apply (simp add: pre_sum_elems_def) (* SH *)
 unfolding Let_def
-apply (elim conjE, intro conjI)
+apply (elim conjE)
 apply (simp add: post_sum_elems_def inv_SeqElems_def 
                   inv_VDMNat_def l_pre_sum_elems l_sum_elems_nat 
-                  pre_sum_elems_def) --"SH"
-apply (simp add: l_inv_SeqElems_Cons, elim conjE)
-apply (cut_tac l_inv_Move_nat1, simp_all)
-apply (intro impI, simp)
-apply (simp add: l_inv_SeqElems_Cons l_inv_Moves_Hd)
-apply (erule conjE)
-by (frule l_inv_Move_nat1, simp) --"SH"
+                  pre_sum_elems_def) (* SH *)
+  apply (simp, elim conjE)
+  unfolding pre_sum_elems_def
+   apply (simp add: l_inv_SeqElems_Cons)
+  apply (elim conjE, intro conjI impI, simp_all)
+  unfolding post_sum_elems_def
+    apply (simp add: l_inv_Moves_Hd)
+    apply (simp add: inv_VDMNat_def l_inv_SeqElems_Cons l_pre_sum_elems l_sum_elems_nat)
+  using l_inv_Move_nat1 l_inv_SeqElems_Cons apply fastforce
+  using l_inv_Move_nat1 l_inv_SeqElems_Cons by fastforce
 
 lemma l_inv_Moves_Cons: 
   "inv_Moves (x # xs) = (inv_Move x \<and> inv_Moves xs)"
 apply (rule iffI)
-using l_inv_Moves_Hd l_inv_Moves_Tl apply blast --"SH"
+using l_inv_Moves_Hd l_inv_Moves_Tl apply blast (* SH *)
 apply (elim conjE)
 unfolding inv_Moves_def post_sum_elems_def Let_def
 apply (elim conjE, intro conjI, simp_all)
-apply (simp add: l_inv_SeqElems_Cons) --"SH"
-apply (simp add: l_inv_SeqElems_Cons pre_sum_elems_def) --"SH"
-apply (simp add: l_inv_SeqElems_Cons) --"SH"
-using inv_VDMNat_def l_inv_Move_nat1 apply fastforce --"SH"
-using l_inv_Move_nat1 apply fastforce --"SH"
-txt{* Goals not provable when @{term "sum_elems xs = MAX_PILE"}, 
-because @{term "inv_Move x"} enforce @{term "x > (0::int)"} *}
+      apply (simp add:  pre_sum_elems_def) (* SH *)
+      apply (simp add: l_inv_SeqElems_Cons)
+   apply (simp add: l_inv_SeqElems_Cons pre_sum_elems_def)
+  using inv_VDMNat_def l_inv_Move_nat1 apply force
+  nitpick[user_axioms=true]
+txt\<open> Goals not provable when @{term "sum_elems xs = MAX_PILE"}, 
+because @{term "inv_Move x"} enforce @{term "x > (0::int)"} \<close>
 oops
 
 (*<*) thm l_moves_left_nat l_inv_Moves_Hd l_inv_Moves_Tl (*>*)
-text {* Lemmas proved as a result of first attempt:
+text \<open> Lemmas proved as a result of first attempt:
 
 \begin{enumerate}
   \item[1.a] @{term "moves_left s"} is @{typ \<nat>} for valid moves @{thm[display] l_moves_left_nat}
@@ -1293,25 +1335,25 @@ Let's see if the lemma shape is working (i.e. it will be used by Isabelle).
 \begin{enumerate}
   \item[2] Using lemmas:~layered expansion followed by simplification with lemmas.
 \end{enumerate}
-*}
+\<close>
 
 theorem PO_best_move_sat_obl0
-txt {* $\cdots$ *}(*<*)
+txt \<open> $\cdots$ \<close>(*<*)
 unfolding PO_best_move_sat_obl0_def pre_best_move0_def post_best_move0_def 
 apply simp
-unfolding pre_moves_left_def post_moves_left0_def
+unfolding pre_moves_left_def post_moves_left_def
 apply simp
 unfolding pre_sum_elems_def post_sum_elems_def
 apply simp
 unfolding  inv_VDMNat_def 
-apply (intro allI impI conjI) --"or apply auto"
+apply (intro allI impI conjI) (*or apply auto*)
 apply (rule_tac x=0 in exI)
 apply simp
 apply (intro conjI)
 find_theorems "_ \<noteq> []" name:Nim (*>*)
-apply (simp add: l_moves_left_nat) --"SH"
-txt {* Yes! The lemma discharged the first suggoal, and \textsf{sledgehammer} found it.
- *}
+apply (simp add: l_moves_left_nat) (* SH *)
+txt \<open> Yes! The lemma discharged the first suggoal, and \textsf{sledgehammer} found it.
+ \<close>
 oops
 
 (* TODO: explain? Tried an unprovable goal to finish the proof... ?
@@ -1320,7 +1362,7 @@ lemma l_moves_left_ms_not_empty: "inv_Moves ms \<Longrightarrow> ms \<noteq> [] 
 sorry 
 
 theorem PO_best_move_sat_obl0
-txt {* $\cdots$ *} (*<*)
+txt \<open> $\cdots$ \<close> (*<*)
 unfolding PO_best_move_sat_obl0_def pre_best_move0_def post_best_move0_def 
 apply simp
 unfolding pre_moves_left_def post_moves_left0_def
@@ -1328,22 +1370,22 @@ apply simp
 unfolding pre_sum_elems_def post_sum_elems_def
 apply simp
 unfolding  inv_VDMNat_def 
-apply (intro allI impI conjI) --"or apply auto"
+apply (intro allI impI conjI) (* or apply auto *)
 apply (rule_tac x=0 in exI)
 apply simp
 apply (intro conjI)
 find_theorems "_ \<noteq> []" name:Nim (*>*)
-apply (simp add: l_moves_left_nat) --"SH"
-apply (simp add: l_moves_left_ms_not_empty) --"SH"
-by (simp add: l_moves_left_nat) --"SH" 
+apply (simp add: l_moves_left_nat) (* SH *)
+apply (simp add: l_moves_left_ms_not_empty) (* SH *)
+by (simp add: l_moves_left_nat) (* SH *) 
 *)
 
-text {* Next we define the PO of @{term best_move} with new post condition @{term post_best_move}, 
+text \<open> Next we define the PO of @{term best_move} with new post condition @{term post_best_move}, 
 yet with the old precondition @{term pre_best_move0}. 
 \begin{enumerate}
   \item[3] revised definition of @{term post_best_move} + using lemmas: \textcolor{red}{\textbf{success?!}}
 \end{enumerate}
-*}
+\<close>
 
 definition
   PO_best_move_sat_obl1 :: "\<bool>"
@@ -1351,7 +1393,7 @@ where
   "PO_best_move_sat_obl1 \<equiv> \<forall> ms . inv_Moves ms \<longrightarrow> pre_best_move0 ms \<longrightarrow> (\<exists> r . post_best_move ms r)"
 
 theorem PO_best_move_sat_obl1
-txt {* $\cdots$ *} (*<*)
+txt \<open> $\cdots$ \<close> (*<*)
 unfolding PO_best_move_sat_obl1_def pre_best_move0_def post_best_move_def 
 apply simp
 unfolding pre_moves_left_def post_moves_left_def
@@ -1359,20 +1401,20 @@ apply simp
 unfolding pre_sum_elems_def post_sum_elems_def
 apply simp
 unfolding inv_VDMNat_def 
-apply (intro allI impI conjI) --"or apply auto"
+apply (intro allI impI conjI) (* or apply auto *)
 apply (rule_tac x=0 in exI)
 apply simp
 apply (intro conjI) (*>*)
-txt {* @{subgoals[display,indent=0]}
+txt \<open> @{subgoals[display,indent=0]}
   With the updated definition, and proved lemmas, we get different subgoals, all dischargeble
   by \textsf{sledgehammer}.  
-*}
-apply (simp add: l_moves_left_nat) --"SH"
-apply (simp add: l_sum_elems_nat) --"SH"
-using l_sum_elems_nat1 apply auto[1] --"SH"
-by (simp add: l_moves_left_nat) --"SH"
+\<close>
+apply (simp add: l_moves_left_nat) (* SH *)
+apply (simp add: l_sum_elems_nat) (* SH *)
+using l_sum_elems_nat1 apply auto[1] (* SH *)
+by (simp add: l_moves_left_nat) (* SH *)
 
-text{*  
+text\<open>  
   What is going on? We proved this, shouldn't it mean that @{term pre_best_move0} is okay?
   No because we have an explicit definition as @{thm[display] best_move_def}
   We need to account for that fact and be specific about the witness, which is to 
@@ -1394,7 +1436,7 @@ with the explicit witness in the next attempt.
   \item[4] Lemmas + explicit witness + no revision of @{term post_best_move} 
 \end{enumerate}
 
-*}
+\<close>
 
 definition
   PO_best_move_sat_obl2 :: "\<bool>"
@@ -1405,41 +1447,42 @@ where
 theorem PO_best_move_sat_obl2
 unfolding PO_best_move_sat_obl2_def pre_best_move0_def post_best_move0_def
 apply (intro allI impI conjI, elim conjE, simp_all)
-unfolding post_moves_left0_def pre_moves_left_def post_sum_elems_def
+unfolding post_moves_left_def pre_moves_left_def post_sum_elems_def
 apply (simp_all)
-txt{* @{subgoals[display,indent=0]}
-   This suggests a trivial lemma about @{term inv_VDMNat} to avoid multiple goals *}
+txt\<open> @{subgoals[display,indent=0]}
+   This suggests a trivial lemma about @{term inv_VDMNat} to avoid multiple goals \<close>
 unfolding inv_VDMNat_def
-apply (simp add: l_moves_left_nat) --"SH"
+apply (simp add: l_moves_left_nat) (* SH *)
 apply (intro conjI)
-apply (simp add: l_moves_left_nat) --"SH"
-apply (simp add: pre_sum_elems_def)--"SH"
-apply (simp add: l_moves_left_nat) --"SH"
-txt{* @{subgoals[display,indent=0]}
+apply (simp add: l_moves_left_nat) (* SH *)
+  apply (simp add: pre_sum_elems_def)(* SH *)
+  apply (simp add: l_sum_elems_nat)
+  apply (simp add: l_pre_sum_elems_sat)
+txt\<open> @{subgoals[display,indent=0]}
    The first subgoal is not provable because @{term "moves_left ms"} can be $0$!
    We can create another lemma for the final subgoal using facts about remainder
-   using theorem search to find @{thm zmod_le_nonneg_dividend}. *}
+   using theorem search to find @{thm zmod_le_nonneg_dividend}. \<close>
 find_theorems "_ mod _ \<le> _"
 oops
 
-text {* Let us create the lemmas suggested by the previous proof. *}
+text \<open> Let us create the lemmas suggested by the previous proof. \<close>
 
 lemma l_inv_VDMNat_moves_left: 
   "inv_Moves ms \<Longrightarrow> inv_VDMNat (moves_left ms)" 
-unfolding inv_VDMNat_def by (simp add: l_moves_left_nat)  --"SH"
+unfolding inv_VDMNat_def by (simp add: l_moves_left_nat)  (* SH *)
 
 lemma l_nim_mod_prop: 
   "x \<ge> 0 \<Longrightarrow> (x - (1::int)) mod y \<le> x" (*nitpick[user_axioms]*)
 quickcheck
-txt {* This is not provable with $x=0, y=2$. What we want is 
+txt \<open> This is not provable with $x=0, y=2$. What we want is 
   to use it for @{thm[display] zmod_le_nonneg_dividend[of "moves_left s" "MAX_MOV"]}
   We need to tighten our assumptions.
-*} (*<*)thm zmod_le_nonneg_dividend[of "moves_left s" "MAX_MOV"](*>*)
+\<close> (*<*)thm zmod_le_nonneg_dividend[of "moves_left s" "MAX_MOV"](*>*)
 oops
 
 lemma l_nim_mod_prop: 
   "x > 0 \<Longrightarrow> (x - (1::int)) mod y \<le> x" 
-by (smt zmod_le_nonneg_dividend) --"SH"
+by (smt zmod_le_nonneg_dividend) (* SH *)
 
 lemma l_moves_left_prop: 
   "inv_Moves ms \<Longrightarrow> pre_sum_elems ms \<Longrightarrow> (ms \<noteq> []) = (0 < moves_left ms)"
@@ -1453,7 +1496,7 @@ apply (cut_tac l_sum_elems_notempty,simp_all+)
 (* MISTAKE: second goal is not provable. There is a problem with moves_left ms > 0, fixed post_moves_left above *)
 oops
 
-text {* Proved lemmas:
+text \<open> Proved lemmas:
 \begin{enumerate}
   \item[4.a] No need to expand @{term inv_VDMNat} for @{term "moves_left ms"} result; @{thm[display] l_inv_VDMNat_moves_left}
   \item[4.b] Remainder property of Nim game. @{thm[display] l_nim_mod_prop}
@@ -1465,29 +1508,30 @@ Failed lemmas:
 \end{enumerate}
 
 Let us try again with the new lemmas.
-*}
+\<close>
 
 theorem PO_best_move_sat_obl2
 unfolding PO_best_move_sat_obl2_def pre_best_move0_def post_best_move0_def
 apply (intro allI impI conjI, elim conjE, simp_all)
-unfolding post_moves_left0_def pre_moves_left_def post_sum_elems_def
+unfolding post_moves_left_def pre_moves_left_def post_sum_elems_def
 apply (simp_all add: l_inv_VDMNat_moves_left)
 unfolding inv_VDMNat_def
 apply (simp, intro conjI)
-apply (simp add: pre_sum_elems_def)--"SH"
+  apply (simp add: pre_sum_elems_def)(* SH *)
+  apply (simp add: l_sum_elems_nat)
 defer
 apply (rule l_nim_mod_prop)
-txt{* @{subgoals[display,indent=0]} 
-  Unprovable part boils down to @{term "moves_left ms"} not being @{typ \<nat>}$_1$. *}
+txt\<open> @{subgoals[display,indent=0]} 
+  Unprovable part boils down to @{term "moves_left ms"} not being @{typ \<nat>}$_1$. \<close>
 oops
 
-text {*
+text \<open>
 With the new lemmas for the explicit witness proved, let us now change the post condition.
 
 \begin{enumerate}
   \item[5] Revised definition @{term post_best_move} + lemmas + explicit witness
 \end{enumerate}
-*}
+\<close>
 
 definition
   PO_best_move_sat_obl3 :: "\<bool>"
@@ -1502,11 +1546,11 @@ unfolding post_moves_left_def pre_moves_left_def post_sum_elems_def
 apply (simp_all add: l_inv_VDMNat_moves_left)
 unfolding inv_VDMNat_def
 apply simp
-apply (simp add: inv_VDMNat_def l_pre_sum_elems l_sum_elems_nat pre_sum_elems_def) --"SH"
+apply (simp add: inv_VDMNat_def l_pre_sum_elems l_sum_elems_nat pre_sum_elems_def) (* SH *)
 apply (rule l_nim_mod_prop)
-txt{* @{subgoals[display,indent=0]} 
+txt\<open> @{subgoals[display,indent=0]} 
   From the failure, let us try and prove the missing lemma.
-*}
+\<close>
 oops
 
 (*<*)
@@ -1521,15 +1565,11 @@ apply (simp add: l_inv_Moves_Tl)
 find_theorems "pre_sum_elems (_ # _)"
 unfolding pre_sum_elems_def
 find_theorems "inv_SeqElems _ (_ # _)"
-apply (simp add: l_inv_SeqElems_Cons)
-apply (erule conjE)
 find_theorems "inv_Move _ \<Longrightarrow> _"
-apply (frule l_inv_Move_nat1)
 find_theorems "0 \<le> sum_elems _"
 apply (frule l_sum_elems_nat)
-apply (case_tac ms)
-apply (simp add: inv_Move_def) --"SH"
-apply simp
+  apply (case_tac ms)
+  apply (simp add: inv_Move_def l_inv_SeqElems_Cons)
 oops
 (*>*)
 
@@ -1537,25 +1577,24 @@ lemma l_moves_left_nat1:
   "inv_Moves ms \<and> pre_sum_elems ms \<Longrightarrow> 0 < moves_left ms"
 unfolding  pre_sum_elems_def moves_left_def
 apply (induct ms, simp_all, elim conjE)
-apply (simp add: l_inv_Moves_Tl l_inv_SeqElems_Cons)
-apply (elim conjE)
-apply (frule l_inv_Move_nat1) 
-apply (frule l_sum_elems_nat)
-txt {* Goal is @{term False}, yet easier to see with generalised aruments *}
+apply (simp add: l_inv_Moves_Tl)
+  apply (frule l_sum_elems_nat)
+  apply simp
+txt \<open> Goal is @{term False}, yet easier to see with generalised aruments \<close>
 oops
 
 lemma "0 \<le> x \<Longrightarrow> 0 < a \<Longrightarrow> 0 < y - (x::int) \<Longrightarrow> 0 < y - (a + x)"
---"qc: x=0,y=1,a=1"
+(*qc: x=0,y=1,a=1*)
 oops
 
-text {*
+text \<open>
   Now we see what the problem is:~@{term best_move} is missing the precondition about
   @{term moves_left} being non-zero for the explicit witness, and leads to our final attempt.
 
 \begin{enumerate}
   \item[6] Revised definitions @{term pre_best_move} and @{term post_best_move} + lemmas + explicit witness
 \end{enumerate}
-*}
+\<close>
 
 definition
   PO_best_move_sat_obl :: "\<bool>"
@@ -1575,28 +1614,28 @@ apply (intro allI impI conjI, elim conjE, simp_all)
 unfolding inv_VDMNat_def
 apply simp
 unfolding post_moves_left_def pre_moves_left_def post_sum_elems_def
-apply (intro conjI, elim conjE,simp_all)
-apply (simp add: l_inv_VDMNat_moves_left) --"SH"
-apply (simp add: pre_sum_elems_def) --"SH"
-apply (meson inv_Moves_def post_sum_elems_def) --"SH"
+apply (intro conjI impI, elim conjE,simp_all)
+apply (simp add: l_inv_VDMNat_moves_left) (* SH *)
+apply (simp add: pre_sum_elems_def) (* SH *)
+apply (meson inv_Moves_def post_sum_elems_def) (* SH *)
   (* Various options to take, some using our lemmas:
       "z3": Try this: apply (simp add: inv_VDMNat_def l_sum_elems_nat pre_sum_elems_def) (0.7 ms). 
       "cvc4": Try this: apply (simp add: inv_VDMNat_def l_sum_elems_nat pre_sum_elems_def) (0.8 ms). 
       "spass": Try this: apply (meson inv_Moves_def post_sum_elems_def) (22 ms).*)
-apply (simp add: l_pre_sum_elems_sat) --"SH"
-by (simp add: l_nim_mod_prop) --"SH"
+apply (simp add: l_pre_sum_elems_sat) (* SH *)
+by (simp add: l_nim_mod_prop) (* SH *)
 
-text {*
+text \<open>
   Finally we managed to prove that the adjusted/corrected definition of @{term best_move} pre and
   post conditions are now appropriate and make sense with the chosen specification, as well
   as the explicit definition. Auxiliary lemmas help \textsf{sledgehammer} find proofs.
   This illustrates how proof ensures models are fit for purpose. 
-*}
+\<close>
 
 (*-----------------------------------------------------------------------*)
-subsection {* @{term max} and @{term min} *}
+subsection \<open> @{term max} and @{term min} \<close>
 
-text{*
+text\<open>
 \begin{vdmsl}[breaklines=true]
 min: int * int -> int
 min(x,y) == if (x < y) then x else y;
@@ -1604,20 +1643,20 @@ min(x,y) == if (x < y) then x else y;
 max: int * int -> int
 max(x,y) == if (x > y) then x else y;
 \end{vdmsl}
-*}
+\<close>
 
-text{* Isabelle already defines these functions and we omit them here. *}
+text\<open> Isabelle already defines these functions and we omit them here. \<close>
 
 (*-----------------------------------------------------------------------*)
-subsection {* @{term flip_current_player} *}
+subsection \<open> @{term flip_current_player} \<close>
 
-text{*
+text\<open>
 \begin{vdmsl}[breaklines=true]
 flip_current_player: Player -> Player
 flip_current_player(p) == if (p = <P1>) then <P2> else <P1>
 post p <> RESULT;
 \end{vdmsl}
-*}
+\<close>
 
 definition
   flip_current_player :: "Player \<Rightarrow> Player "
@@ -1625,7 +1664,7 @@ where
   "flip_current_player p \<equiv> (if (p = P1) then P2 else P1)"
 
 (*+++++++++++++++++++++++++++++++++++++++++++++++++++++++++++++++++++++++*)
-subsubsection {* Specification *}
+subsubsection \<open> Specification \<close>
 
 definition
   post_flip_current_player :: "Player \<Rightarrow> Player \<Rightarrow> \<bool>"
@@ -1634,7 +1673,7 @@ where
 
 
 (*+++++++++++++++++++++++++++++++++++++++++++++++++++++++++++++++++++++++*)
-subsubsection {* Satisfiability PO *}
+subsubsection \<open> Satisfiability PO \<close>
 
 definition
   PO_flip_current_player_sat_obl :: "\<bool>"
@@ -1644,7 +1683,7 @@ where
 
 theorem PO_flip_current_player_sat_obl 
 unfolding PO_flip_current_player_sat_obl_def post_flip_current_player_def 
-by (metis Player.distinct(1))--"SH"
+by (metis Player.distinct(1))(* SH *)
 
 definition
   PO_flip_current_player_sat_exp_obl :: "\<bool>"
@@ -1655,12 +1694,12 @@ where
 theorem PO_flip_current_player_sat_exp_obl 
 unfolding PO_flip_current_player_sat_exp_obl_def post_flip_current_player_def 
         flip_current_player_def
-by simp --"SH"
+by simp (* SH *)
 
 (*************************************************************************)
-section {* VDM state *}
+section \<open> VDM state \<close>
 
-text{*
+text\<open>
 \begin{vdmsl}[breaklines=true]
 state Nim of
 	limit: Move
@@ -1678,40 +1717,40 @@ inv mk_Nim(limit, current, moves) ==
 init nim == nim = mk_Nim(MAX_MOV, first_player(), [])
 end 
 \end{vdmsl}
-*}
+\<close>
 
-text {*
+text \<open>
   We use records to represent the VDM state. You can also use cartesian product or tuples.
   You need to represent the state invariant, its initialisation, and the result of the
   invariant on the given initial values.  
-*}
+\<close>
 
 record NimSt =
   limit :: Move
   current :: Player
   moves :: Moves
 
-text {*
+text \<open>
   VDM records field access ($x.moves$) is defined in Isabelle through functions (@{term "moves x"}),
   whereas record constants ($mkNimSt(l, c, m)$) are defined in Isabelle as @{term "\<lparr> limit = l, current = c, moves = m \<rparr>"}.
   So, for instance, the result of
 
-  @{term[display] "moves (| limit = MAX_MOV, current = P1, moves = [(1::int),2] |)"}
+  @{term[display] "moves \<lparr> limit = MAX_MOV, current = P1, moves = [(1::int),2] \<rparr>"}
 
   is the sequence @{value "[1,(2::int)]"}. 
-*}
+\<close>
 
 (*-----------------------------------------------------------------------*)
-subsection {* State invariant *}
+subsection \<open> State invariant \<close>
 
-text {*
+text \<open>
   For the state invariant we define a curried function with its components, checking
   the appropriate types first, and next the state invariant itself. Note that if the
   invariant makes use of auxiliary function definitions, it is implicitly adhering to
   those functions specifications as well (e.g.~pre/post for @{term isFirst} and 
   @{term fair_play}).
   Finally, we also define a version of the invariant on the state record itself. 
-*}
+\<close>
 
 definition 
   inv_Nim_flat :: "Move \<Rightarrow> Player \<Rightarrow> Moves \<Rightarrow> \<bool>"
@@ -1725,37 +1764,47 @@ definition
   inv_Nim :: "NimSt \<Rightarrow> \<bool>"
 where
   "inv_Nim st \<equiv> inv_Nim_flat (limit st) (current st) (moves st)"
-
+                      
 (*-----------------------------------------------------------------------*)
-subsection {* State initialisation *}
+subsection \<open> State initialisation \<close>
 
-text {*
+text \<open>
   Initialisation is defined with an Isabelle record value.
   This of course must enforce the invariant as its postcondition.
-*}
+\<close>
 
 definition 
   init_Nim :: "NimSt"
 where
   "init_Nim \<equiv> \<lparr> limit = MAX_MOV, current = P1, moves = [] \<rparr>"
-
-definition
-  post_init_Nim :: "\<bool>"
-where
-  "post_init_Nim \<equiv> inv_Nim init_Nim"
    
 (*-----------------------------------------------------------------------*)
-subsection {* State satisfiability PO *}
+subsection \<open> State satisfiability PO \<close>
   
 definition 
   PO_Nim_initialise_sat_obl :: "\<bool>"
 where
-  "PO_Nim_initialise_sat_obl \<equiv> True"
-  
-(*************************************************************************)
-section {* VDM operations *}
+  "PO_Nim_initialise_sat_obl \<equiv> inv_Nim init_Nim"
 
-text {*
+theorem PO_Nim_initialise_sat_obl
+  unfolding  PO_Nim_initialise_sat_obl_def inv_Nim_def init_Nim_def inv_Nim_flat_def
+  apply simp
+  unfolding inv_Move_def inv_Moves_def
+  apply auto
+  unfolding pre_fair_play_def post_fair_play_def pre_who_plays_next_def post_who_plays_next_def
+  unfolding pre_sum_elems_def post_sum_elems_def inv_Move_def inv_VDMNat_def inv_VDMNat1_def
+        apply auto
+  unfolding inv_Moves_def isFirst_def inv_Player_def
+  apply auto
+  unfolding pre_sum_elems_def post_sum_elems_def inv_Move_def inv_VDMNat_def inv_VDMNat1_def
+    apply auto
+  unfolding fair_play_def who_plays_next_def len_def
+  by auto
+
+(*************************************************************************)
+section \<open> VDM operations \<close>
+
+text \<open>
   VDM operations, in so far as Isabelle is concerned, only require pre/post. That is because
   these are the parts that appear in the the proof obligations to be discharged. You might also
   want to define the explicit definition (e.g. the how), but is not strictly necessary. 
@@ -1767,12 +1816,107 @@ text {*
   accordingly. Note that you need to check type invariants, as well as auxiliary function pre/post 
   conditions on the appropriate arguments. For instance, @{term post_naive_choose_move} below references
   to @{term "moves_left ms"} is referring to the VDM after state (@{text "moves ast"}) of @{term Moves}.
-*}
+\<close>
 
 (*-----------------------------------------------------------------------*)
-subsection {* @{term naive_choose_move} operation *}
+subsection \<open> @{term who_won} operation \<close>
 
-text{*
+text\<open>
+\begin{vdmsl}[breaklines=true]
+-- who won is determined by who played more moves? 
+who_won() w: Player ==
+	return current -- who_plays_next(moves)
+ext rd current, moves
+pre isFirst(first_player())
+post (who_won_invariant(w, moves) 
+			and 
+			-- last save flipped loser and put winner as current
+			w = current)
+\end{vdmsl}
+\<close>
+
+(*+++++++++++++++++++++++++++++++++++++++++++++++++++++++++++++++++++++++*)
+subsubsection \<open> Specification \<close>
+
+definition
+  pre_who_won :: "NimSt \<Rightarrow> \<bool>"
+where
+  "pre_who_won bst \<equiv> inv_Nim bst \<and> isFirst P1"
+
+definition
+  post_who_won :: "Player \<Rightarrow> NimSt \<Rightarrow> NimSt \<Rightarrow> \<bool>"
+where
+  "post_who_won w bst ast \<equiv>
+     pre_who_won bst \<longrightarrow> 
+     inv_Player w \<and> inv_Nim ast \<and>
+     (current bst) = (current ast) \<and>
+     (limit bst) = (limit ast) \<and>
+     (moves bst) = (moves ast) \<and>
+     pre_who_won_invariant w (moves ast) (limit ast) \<and>
+     post_who_won_invariant w (moves ast) (limit ast) (who_won_invariant w (moves ast) (limit ast)) \<and>
+     (who_won_invariant w (moves ast) (limit ast)) \<and>
+     w = current ast"
+
+(*+++++++++++++++++++++++++++++++++++++++++++++++++++++++++++++++++++++++*)
+subsubsection \<open> Implementation \<close>
+
+definition
+  who_won :: "NimSt \<Rightarrow> Player"
+where
+  "who_won bst \<equiv> (current bst)"
+
+definition
+  who_won_complete :: "NimSt \<Rightarrow> (NimSt \<times> Player)"
+where
+  "who_won_complete bst \<equiv> (bst, (current bst))"
+
+
+(*-----------------------------------------------------------------------*)
+subsection \<open> @{term tally} operation \<close>
+
+text\<open>
+\begin{vdmsl}[breaklines=true]
+tally() ==
+	 (print("\nPlayer ");print(who_won());println(" won! Play finished with:");
+	  print("\tP1 moves = ");println(moves_of(moves, isFirst(<P1>)));
+	  print("\tP2 moves = ");println(moves_of(moves, isFirst(<P2>)));
+	 )
+ext rd current, moves;	
+\end{vdmsl}
+\<close>
+
+(*+++++++++++++++++++++++++++++++++++++++++++++++++++++++++++++++++++++++*)
+subsubsection \<open> Specification \<close>
+
+definition
+  pre_tally :: "NimSt \<Rightarrow> \<bool>"
+where
+  "pre_tally bst \<equiv> inv_Nim bst \<and> pre_who_won bst"
+
+definition
+  post_tally :: "NimSt \<Rightarrow> NimSt \<Rightarrow> \<bool>"
+where
+  "post_tally bst ast \<equiv>
+     pre_tally bst \<longrightarrow>  
+     inv_Nim ast  \<and>  post_who_won (current ast) bst ast"
+
+(*+++++++++++++++++++++++++++++++++++++++++++++++++++++++++++++++++++++++*)
+subsubsection \<open> Implementation \<close>
+
+text \<open> 
+  We define tally in VDM to illustrate the use of sequential composition. 
+  We will not show I/O in Isabelle.  
+\<close>
+
+definition
+  tally :: "NimSt \<Rightarrow> NimSt"
+where
+  "tally bst \<equiv> (let p = who_won bst in bst)"
+
+(*-----------------------------------------------------------------------*)
+subsection \<open> @{term naive_choose_move} operation \<close>
+
+text\<open>
 \begin{vdmsl}[breaklines=true]
 naive_choose_move() r: Move == 
 	-- naive choice: from 1 up to MAX_MOV or else amount left, presuming there are at least the last
@@ -1783,13 +1927,13 @@ post
 	-- might be = in the case of the loosing play
 	r <= moves_left(moves);
 \end{vdmsl}
-*}
+\<close>
 
 (*+++++++++++++++++++++++++++++++++++++++++++++++++++++++++++++++++++++++*)
-subsubsection {* Specification *}
+subsubsection \<open> Specification \<close>
 
-text {* Notice that @{term moves_left} in the postcondition is applied to the 
-after state  (e.g. @{term "moves ast"}). *}
+text \<open> Notice that @{term moves_left} in the postcondition is applied to the 
+after state  (e.g. @{term "moves ast"}). \<close>
 
 definition
   pre_naive_choose_move :: "NimSt \<Rightarrow> \<bool>"
@@ -1798,29 +1942,27 @@ where
       inv_Nim bst \<and> 
       (let ms = (moves bst) in
         pre_moves_left ms \<and> 
-        post_moves_left ms (moves_left ms) \<and> 
-        {1 .. (min MAX_MOV (moves_left ms))} \<noteq> {} \<and>
         moves_left ms > 0)"
 
 definition
   post_naive_choose_move :: "Move \<Rightarrow> NimSt \<Rightarrow> NimSt \<Rightarrow> \<bool>"
 where
-  "post_naive_choose_move RESULT bst ast \<equiv>
-      inv_Move RESULT \<and> inv_Nim bst \<and> inv_Nim ast \<and> 
-      (let ms = (moves ast) in
-        pre_moves_left ms \<and> 
-        post_moves_left ms (moves_left ms) \<and>
-        RESULT \<le> moves_left (moves ast))"
+  "post_naive_choose_move r bst ast \<equiv>
+      pre_naive_choose_move bst \<longrightarrow>
+      inv_Move r \<and> inv_Nim ast \<and> 
+      (let bms = (moves bst) in
+        post_moves_left bms (moves_left bms) \<and>
+        r \<le> moves_left bms)"
 
 (*+++++++++++++++++++++++++++++++++++++++++++++++++++++++++++++++++++++++*)
-subsubsection {* Implementation *}
+subsubsection \<open> Implementation \<close>
 
-text {* 
+text \<open> 
   The implementation uses VDM's non deterministic (Hilbert's-)choice over a set. 
   It can be encoded with Isabelle's Hilbert's choice operator\footnote{See~\url{https://en.wikipedia.org/wiki/Choice_function}}. 
   Like in VDM, this has the precondition that the underlying set/sequence are not empty.
   Proofs involving Hilbert's choice are tricky/difficult.
-*}
+\<close>
 
 lemma "(SOME m . m \<in> {1 .. MAX_MOV}) > 0"
   find_theorems "SOME _ . _ \<in> _" name:Hilbert
@@ -1837,12 +1979,12 @@ lemma "(SOME m . m \<in> {1 .. (3::int)}) > 0"
   apply (rule someI2)
   by auto
 
-text {*
+text \<open>
   Operations should always return the sate and its result type. You could 
   choose to avoid returning the state if there are no \texttt{ext wr} clauses declared
   (\textit{i.e.}~the operation is read-only and doesn't change the sate). This simplification
   is useful to avoid needing to handle tuples in proofs. I provide both versions for illustrative purposes.
-*}
+\<close>
 
 definition
   naive_choose_move0 :: "NimSt \<Rightarrow> NimSt \<times> Move"
@@ -1856,139 +1998,10 @@ where
   "naive_choose_move st \<equiv>  
     (SOME m . m \<in> {1 .. (min MAX_MOV (moves_left (moves st)))})"
 
-
 (*-----------------------------------------------------------------------*)
-subsection {* @{term first_player_winning_choose_move} operation *}
+subsection \<open> @{term fixed_choose_move} operation \<close>
 
-text{*
-\begin{vdmsl}[breaklines=true]
-first_player_winning_choose_move() r: Move == 
-	-- winning choice: get the best move, unless it's zero, so choose the least worst (1) play
-	return max(1, best_move(moves))
-ext rd moves, current
-pre moves_left(moves) > 0
-post 
-	-- can never be = moves_left(moves) or it would entail loosing?
-	r < moves_left(moves)
-	and
-	-- after playing the chosen move r, the next player has no good move choice
-	will_first_player_win() => best_move(play_move(current, r, moves)) = 0
-	;
-\end{vdmsl}
-*}
-
-(*+++++++++++++++++++++++++++++++++++++++++++++++++++++++++++++++++++++++*)
-subsubsection {* Specification *}
-
-definition
-  pre_first_player_winning_choose_move :: "NimSt \<Rightarrow> \<bool>"
-where
-  "pre_first_player_winning_choose_move bst \<equiv> 
-      inv_Nim bst \<and> pre_moves_left (moves bst) \<and> moves_left (moves bst) > 0"
-
-definition
-  post_first_player_winning_choose_move :: "Move \<Rightarrow> NimSt \<Rightarrow> NimSt \<Rightarrow> \<bool>"
-where
-  "post_first_player_winning_choose_move RESULT bst ast \<equiv>
-      inv_Move RESULT \<and> inv_Nim bst \<and> inv_Nim ast \<and>
-      (let bms = (moves bst) in 
-       let ams = (moves ast) in
-        pre_moves_left ams \<and> post_moves_left ams (moves_left ams) \<and>
-        pre_who_plays_next ams \<and> post_who_plays_next ams (who_plays_next ams) \<and>
-        pre_will_first_player_win \<and>
-        (let ac = (current ast) in
-         let pm = play_move ac RESULT ams in
-         let bm = best_move pm in
-          pre_play_move ac RESULT ams \<and>
-          post_play_move ac RESULT ams pm \<and>
-          pre_best_move pm \<and> post_best_move pm (best_move pm) \<and>
-
-          RESULT < moves_left ams \<and>
-          will_first_player_win \<and>
-          (isFirst (who_plays_next ams) \<longrightarrow> best_move pm = 0)
-        ))"
-
-(*+++++++++++++++++++++++++++++++++++++++++++++++++++++++++++++++++++++++*)
-subsubsection {* Implementation *}
-
-definition
-  first_player_winning_choose_move :: "NimSt \<Rightarrow> Move"
-where
-  "first_player_winning_choose_move st \<equiv> max 1 (best_move (moves st))"
-
-(*+++++++++++++++++++++++++++++++++++++++++++++++++++++++++++++++++++++++*)
-subsubsection {* Example PO: operation satisfiability *}
-
-text {*
-	The satisfiability proof obligation of an operation $Op$ under state $St$ is:
-	
-	@{term[display] "\<forall> input \<in> Type . \<forall> bst \<in> State . pre_Op input bst \<longrightarrow> 
-	      (\<exists> output \<in> Type . \<exists> ast \<in> State .  post_Op input output bst ast)"}
-	
-	That is, given any input and before state satisfying their invariants, if the precondition holds, then 
-	find witnesses for the output and after state, such that the postcondition holds. 
-	Operations without inputs or outputs can be declared similarly without the parameters.
-	Operations with explicit definition have the witness choice fixed for the existential quantifiers.
-	
-	Overture PO generator (POG) produces different versions of the satisfiability PO, 
-	depending on the kind of VDM declaration used (\textit{e.g.}~implicit, explicit, extended). 
-	In essence, the POG expand/simplifies definitions, as well as take advantage of explicit 
-	specification statements as witnesses to existential quantifiers. In doubt, use the 
-	general template above.
-*}
-
-definition
-  PO_first_player_winning_choose_move_sat_obl :: \<bool>
-where
-  "PO_first_player_winning_choose_move_sat_obl \<equiv> 
-      \<forall> bst . pre_first_player_winning_choose_move bst \<longrightarrow> 
-            (\<exists> RESULT ast . post_first_player_winning_choose_move RESULT bst ast)"
-
-definition
-  PO_first_player_winning_choose_move_sat_exp_obl :: \<bool>
-where
-  "PO_first_player_winning_choose_move_sat_exp_obl \<equiv> 
-      \<forall> bst . pre_first_player_winning_choose_move bst \<longrightarrow> 
-        post_first_player_winning_choose_move (max 1 (best_move (moves bst))) bst bst"
-
-text{* As an illustration, a naive attempt at these kind of proofs by simply expanding
-definitions and doing layered simplificaiton will only work if appropriate lemmas
-are in place. Previous proofs of satisfiability of involved functions will also be 
-important in these POs about top-level operations. *}
-
-theorem PO_first_player_winning_choose_move_sat_exp_obl
-unfolding PO_first_player_winning_choose_move_sat_exp_obl_def
-unfolding pre_first_player_winning_choose_move_def
-          post_first_player_winning_choose_move_def Let_def
-apply auto (*
-unfolding inv_Nim_def inv_Nim_flat_def
-          inv_Moves_def inv_SeqElems_def
-          inv_Move_def nat1G0 max_def
-
-          pre_moves_left_def
-          pre_best_move_def
-          pre_best_move0_def
-          post_best_move_def
-          pre_who_plays_next_def
-          pre_fair_play_def
-          pre_play_move_def
-          pre_sum_elems_def
-
-          moves_left_def
-          best_move_def
-          who_plays_next_def
-          fair_play_def
-          play_move_def
-
-          isFirst_def
-          will_first_player_win_def
-apply (intro allI impI, elim conjE) *)
-oops
-
-(*-----------------------------------------------------------------------*)
-subsection {* @{term fixed_choose_move} operation *}
-
-text{*
+text\<open>
 \begin{vdmsl}[breaklines=true]
 fixed_choose_move() r: Move == 
 	return FIXED_PLAY(len moves + 1)
@@ -2009,13 +2022,13 @@ values
 									-- 1 2 1 2 1 2 1 2 1 2
 FIXED_PLAY: Moves = [3,2,2,1,3,2,2,1,3,1];
 \end{vdmsl}
-*}
+\<close>
 
-text {*
+text \<open>
   The @{term FIXED_PLAY} value needs to be declared first as it is used in the coming definition. 
   Also, it needs to satisfy the invariant of @{term Moves} in the precondition of where it appears. 
   We use @{term definition} instead of @{term abbreviation} to avoid expansion in proofs.
-*}
+\<close>
 
 definition
   FIXED_PLAY :: "Moves"
@@ -2028,36 +2041,209 @@ where
   "inv_FIXED_PLAY \<equiv> inv_Moves FIXED_PLAY"
 
 (*+++++++++++++++++++++++++++++++++++++++++++++++++++++++++++++++++++++++*)
-subsubsection {* Specification *}
+subsubsection \<open> Specification \<close>
 
 definition
   pre_fixed_choose_move :: "NimSt \<Rightarrow> \<bool>"
 where
   "pre_fixed_choose_move bst \<equiv> 
-      pre_first_player_winning_choose_move bst"
+      pre_naive_choose_move bst"
 
 definition
   post_fixed_choose_move :: "Move \<Rightarrow> NimSt \<Rightarrow> NimSt \<Rightarrow> \<bool>"
 where
   "post_fixed_choose_move RESULT bst ast \<equiv>
-      post_first_player_winning_choose_move RESULT bst ast"
+      post_naive_choose_move RESULT bst ast"
 
 (*+++++++++++++++++++++++++++++++++++++++++++++++++++++++++++++++++++++++*)
-subsubsection {* Implementation *}
+subsubsection \<open> Implementation \<close>
 
 definition
   fixed_choose_move :: "NimSt \<Rightarrow> Move"
 where
-  "fixed_choose_move st \<equiv> applyVDMSeq FIXED_PLAY (len (moves st) + 1)"
-
+  "fixed_choose_move st \<equiv> FIXED_PLAY $ (len (moves st) + 1)"
 
 (*-----------------------------------------------------------------------*)
-subsection {* @{term save} operation *}
+subsection \<open> @{term first_player_winning_choose_move} operation \<close>
 
-text{*
+text\<open>
+\begin{vdmsl}[breaklines=true]
+first_player_winning_choose_move() r: Move == 
+	-- winning choice: get the best move, unless it's zero, so choose the least worst (1) play
+	return max(1, best_move(moves))
+ext rd moves, current
+pre moves_left(moves) > 0
+post 
+	-- can never be = moves_left(moves) or it would entail loosing?
+	r < moves_left(moves)
+	and
+	-- after playing the chosen move r, the next player has no good move choice
+	will_first_player_win() => best_move(play_move(current, r, moves)) = 0
+	;
+\end{vdmsl}
+\<close>
+
+(*+++++++++++++++++++++++++++++++++++++++++++++++++++++++++++++++++++++++*)
+subsubsection \<open> Specification \<close>
+
+definition
+  pre_first_player_winning_choose_move0 :: "NimSt \<Rightarrow> \<bool>"
+where
+  "pre_first_player_winning_choose_move0 bst \<equiv> 
+      inv_Nim bst \<and> pre_moves_left (moves bst) \<and> moves_left (moves bst) > 0"
+
+definition
+  pre_first_player_winning_choose_move :: "NimSt \<Rightarrow> \<bool>"
+where
+  "pre_first_player_winning_choose_move bst \<equiv> 
+      inv_Nim bst \<and> 
+      pre_moves_left (moves bst) \<and> 
+      pre_best_move (moves bst) \<and> 
+      moves_left (moves bst) > 0 \<and> 
+      best_move (moves bst) > 0"
+
+definition
+  post_first_player_winning_choose_move0 :: "Move \<Rightarrow> NimSt \<Rightarrow> NimSt \<Rightarrow> \<bool>"
+where
+  "post_first_player_winning_choose_move0 RESULT bst ast \<equiv>
+      pre_first_player_winning_choose_move0 bst \<longrightarrow>
+      inv_Move RESULT \<and> inv_Nim ast \<and>
+      (let bms = (moves bst);
+           ams = (moves ast);
+           alim= (limit ast);
+            ac = (current ast);
+           pm = play_move ac RESULT ams;
+          bm = best_move pm
+        in
+        pre_moves_left ams \<and> post_moves_left ams (moves_left ams) \<and>
+        pre_who_plays_next ams \<and> post_who_plays_next ams (who_plays_next ams) \<and>
+        pre_will_first_player_win alim \<and>
+         pre_play_move ac RESULT ams \<and>
+          post_play_move ac RESULT ams pm \<and>
+          pre_best_move pm \<and> post_best_move pm (best_move pm) \<and>
+          
+          (limit bst) = (limit ast) \<and> (current bst) = (current ast) \<and> (moves bst) = (moves ast) \<and> 
+          RESULT < moves_left ams \<and>
+          (will_first_player_win alim \<longrightarrow> best_move pm = 0)
+        )"
+            (* TODO: add limit parameter to best_move ! *)
+
+definition
+  post_first_player_winning_choose_move :: "Move \<Rightarrow> NimSt \<Rightarrow> NimSt \<Rightarrow> \<bool>"
+where
+  "post_first_player_winning_choose_move RESULT bst ast \<equiv>
+      pre_first_player_winning_choose_move bst \<longrightarrow>
+      inv_Move RESULT \<and> inv_Nim ast \<and>
+      (let bms = (moves bst);
+           ams = (moves ast);
+           alim= (limit ast);
+            ac = (current ast);
+           pm = play_move ac RESULT ams;
+          bm = best_move pm
+        in
+        pre_moves_left ams \<and> post_moves_left ams (moves_left ams) \<and>
+        pre_who_plays_next ams \<and> post_who_plays_next ams (who_plays_next ams) \<and>
+        pre_will_first_player_win alim \<and>
+         pre_play_move ac RESULT ams \<and>
+          post_play_move ac RESULT ams pm \<and>
+          pre_best_move pm \<and> post_best_move pm (best_move pm) \<and>
+          (limit bst) = (limit ast) \<and> (current bst) = (current ast) \<and> (moves bst) = (moves ast) \<and> 
+          RESULT < moves_left ams \<and>
+          (will_first_player_win alim \<longrightarrow> best_move pm = 0)
+        )"
+
+(*+++++++++++++++++++++++++++++++++++++++++++++++++++++++++++++++++++++++*)
+subsubsection \<open> Implementation \<close>
+
+definition
+  first_player_winning_choose_move :: "NimSt \<Rightarrow> Move"
+where
+  "first_player_winning_choose_move st \<equiv> best_move (moves st)"
+
+(*+++++++++++++++++++++++++++++++++++++++++++++++++++++++++++++++++++++++*)
+subsubsection \<open> Example PO: operation satisfiability \<close>
+
+text \<open>
+	The satisfiability proof obligation of an operation $Op$ under state $St$ is:
+	
+	@{term[display] "\<forall> input \<in> Type . \<forall> bst \<in> State . pre_Op input bst \<longrightarrow> 
+	      (\<exists> output \<in> Type . \<exists> ast \<in> State .  post_Op input output bst ast)"}
+	
+	That is, given any input and before state satisfying their invariants, if the precondition holds, then 
+	find witnesses for the output and after state, such that the postcondition holds. 
+	Operations without inputs or outputs can be declared similarly without the parameters.
+	Operations with explicit definition have the witness choice fixed for the existential quantifiers.
+	
+	Overture PO generator (POG) produces different versions of the satisfiability PO, 
+	depending on the kind of VDM declaration used (\textit{e.g.}~implicit, explicit, extended). 
+	In essence, the POG expand/simplifies definitions, as well as take advantage of explicit 
+	specification statements as witnesses to existential quantifiers. In doubt, use the 
+	general template above.
+\<close>
+
+definition
+  PO_first_player_winning_choose_move_sat_obl :: \<bool>
+where
+  "PO_first_player_winning_choose_move_sat_obl \<equiv> 
+      \<forall> bst . pre_first_player_winning_choose_move bst \<longrightarrow> 
+            (\<exists> RESULT ast . post_first_player_winning_choose_move RESULT bst ast)"
+
+definition
+  PO_first_player_winning_choose_move_sat_exp_obl0 :: \<bool>
+where
+  "PO_first_player_winning_choose_move_sat_exp_obl0 \<equiv> 
+      \<forall> bst . pre_first_player_winning_choose_move0 bst \<longrightarrow> 
+        post_first_player_winning_choose_move0 (first_player_winning_choose_move  bst) bst bst"
+
+definition
+  PO_first_player_winning_choose_move_sat_exp_obl :: \<bool>
+where
+  "PO_first_player_winning_choose_move_sat_exp_obl \<equiv> 
+      \<forall> bst . pre_first_player_winning_choose_move bst \<longrightarrow> 
+        post_first_player_winning_choose_move (first_player_winning_choose_move  bst) bst bst"
+
+text\<open> As an illustration, a naive attempt at these kind of proofs by simply expanding
+definitions and doing layered simplification will only work if appropriate lemmas
+are in place. Previous proofs of satisfiability of involved functions will also be 
+important in these POs about top-level operations. \<close>
+
+theorem PO_first_player_winning_choose_move_sat_exp_obl
+  unfolding PO_first_player_winning_choose_move_sat_exp_obl_def
+unfolding pre_first_player_winning_choose_move_def
+          post_first_player_winning_choose_move_def Let_def
+apply simp
+unfolding inv_Nim_def inv_Nim_flat_def
+          inv_Moves_def inv_SeqElems_def
+          inv_Move_def max_def
+  apply simp
+  unfolding
+          pre_moves_left_def
+          pre_best_move_def
+          pre_best_move0_def
+          post_best_move_def
+          pre_who_plays_next_def
+          pre_fair_play_def
+          pre_play_move_def
+          pre_sum_elems_def
+  apply simp
+  unfolding  moves_left_def
+          best_move_def
+          who_plays_next_def
+          fair_play_def
+          play_move_def
+  apply simp
+  unfolding  isFirst_def
+          will_first_player_win_def
+  apply safe
+oops
+
+(*-----------------------------------------------------------------------*)
+subsection \<open> @{term save} operation \<close>
+
+text\<open>
 \begin{vdmsl}[breaklines=true]
 save(choice : Move) == 
-	(dcl ms  : Moves := play_move(current, choice, moves),
+	(dcl ms  : Moves  := play_move(current, choice, moves),
 			 next: Player := flip_current_player(current);
 		--flip_player();, see flip_current_player(current) instead
 		-- to keep the fair_play_invariant, we need to change both atomically
@@ -2071,47 +2257,44 @@ save(choice : Move) ==
 ext wr current, moves
 pre pre_play_move(current, choice, moves) 
 post 
-	post_play_move(current, choice, moves~, moves)
+	post_play_move(current~, choice, moves~, moves)
 	and
 	current~ <> current
 \end{vdmsl}
-*}
+\<close>
 
 (*+++++++++++++++++++++++++++++++++++++++++++++++++++++++++++++++++++++++*)
-subsubsection {* Specification *}
+subsubsection \<open> Specification \<close>
 
 definition
   pre_save :: "Move \<Rightarrow> NimSt \<Rightarrow> \<bool>"
 where
   "pre_save choice bst \<equiv> 
       inv_Nim bst \<and> inv_Move choice \<and>
-      (let bc = (current bst) in
-       let bms= (moves bst) in
-      pre_play_move bc choice bms \<and>
-      post_play_move bc choice bms 
-                     (play_move bc choice bms))"
+      (let bc = (current bst);
+           bms= (moves bst) 
+       in
+           pre_play_move bc choice bms)"
 
 definition
   post_save :: "Move \<Rightarrow> NimSt \<Rightarrow> NimSt \<Rightarrow> \<bool>"
 where
   "post_save choice bst ast \<equiv> 
       inv_Nim bst \<and> inv_Nim ast \<and> inv_Move choice \<and> 
-      (let bc = (current bst) in 
-       let ac = (current ast) in
-       let bms= (moves bst) in 
-       let ams= (moves ast) in
-       pre_play_move bc choice bms \<and>
-       post_play_move bc choice bms (play_move bc choice bms) \<and>
-       post_flip_current_player bc (flip_current_player bc) \<and>
-
-       pre_play_move ac choice ams \<and>
-       post_play_move ac choice bms ams 
-      )"
+      (let bc = (current bst);
+           ac = (current ast);
+           bms= (moves bst);
+           ams= (moves ast) in
+         ams = (play_move bc choice bms) \<and>
+         post_play_move bc choice bms ams \<and>
+         post_flip_current_player bc (flip_current_player bc) \<and>
+         bc \<noteq> ac
+       )"
 
 (*+++++++++++++++++++++++++++++++++++++++++++++++++++++++++++++++++++++++*)
-subsubsection {* Implementation *}
+subsubsection \<open> Implementation \<close>
 
-text {*
+text \<open>
   For read-write operations, the after state must be returned together with any result value
   as a tupple or extended record. Like with read-only operations, if result is void, then just 
   the state is enough as a result type to avoid needing to handle tuples unnecessarily.
@@ -2121,7 +2304,7 @@ text {*
   statements (\textit{i.e.}~there aren't any state updates as such:~a new state is built and
   returned as a result). You can either rebuild the whole state as a new record (@{term save}) 
   or use record update syntax (@{term save2}). 
-*}
+\<close>
 
 definition
   save :: "Move \<Rightarrow> NimSt \<Rightarrow> NimSt"
@@ -2140,94 +2323,10 @@ where
          bst \<lparr> current := next, moves := ms \<rparr>)"
 
 (*-----------------------------------------------------------------------*)
-subsection {* @{term who_won} operation *}
-
-text{*
-\begin{vdmsl}[breaklines=true]
--- who won is determined by who played more moves? 
-who_won() w: Player ==
-	return current -- who_plays_next(moves)
-ext rd current, moves
-pre isFirst(first_player())
-post (who_won_invariant(w, moves) 
-			and 
-			-- last save flipped loser and put winner as current
-			w = current)
-\end{vdmsl}
-*}
-
-(*+++++++++++++++++++++++++++++++++++++++++++++++++++++++++++++++++++++++*)
-subsubsection {* Specification *}
-
-definition
-  pre_who_won :: "NimSt \<Rightarrow> \<bool>"
-where
-  "pre_who_won bst = inv_Nim bst"
-
-definition
-  post_who_won :: "Player \<Rightarrow> NimSt \<Rightarrow> NimSt \<Rightarrow> \<bool>"
-where
-  "post_who_won RESULT bst ast \<equiv>
-     inv_Nim bst \<and> inv_Nim ast \<and>
-     (let ams = (moves ast) in
-       pre_who_won_invariant RESULT ams \<and>
-       post_who_won_invariant RESULT ams (who_won_invariant RESULT ams))"
-
-(*+++++++++++++++++++++++++++++++++++++++++++++++++++++++++++++++++++++++*)
-subsubsection {* Implementation *}
-
-definition
-  who_won :: "NimSt \<Rightarrow> Player"
-where
-  "who_won bst \<equiv> (current bst)"
-
-(*-----------------------------------------------------------------------*)
-subsection {* @{term tally} operation *}
-
-text{*
-\begin{vdmsl}[breaklines=true]
-tally() ==
-	 (print("\nPlayer ");print(who_won());println(" won! Play finished with:");
-	  print("\tP1 moves = ");println(moves_of(moves, isFirst(<P1>)));
-	  print("\tP2 moves = ");println(moves_of(moves, isFirst(<P2>)));
-	 )
-ext rd current, moves;	
-\end{vdmsl}
-*}
-
-(*+++++++++++++++++++++++++++++++++++++++++++++++++++++++++++++++++++++++*)
-subsubsection {* Specification *}
-
-definition
-  pre_tally :: "NimSt \<Rightarrow> \<bool>"
-where
-  "pre_tally bst \<equiv> inv_Nim bst \<and> pre_who_won bst"
-
-definition
-  post_tally :: "NimSt \<Rightarrow> NimSt \<Rightarrow> \<bool>"
-where
-  "post_tally bst ast \<equiv>
-     inv_Nim bst \<and> inv_Nim ast \<and> pre_who_won bst \<and> 
-     post_who_won (current ast) bst ast"
-
-(*+++++++++++++++++++++++++++++++++++++++++++++++++++++++++++++++++++++++*)
-subsubsection {* Implementation *}
-
-text {* 
-  We define tally in VDM to illustrate the use of sequential composition. 
-  We will not show I/O in Isabelle.  
-*}
-
-definition
-  tally :: "NimSt \<Rightarrow> NimSt"
-where
-  "tally bst \<equiv> (let p = who_won bst in bst)"
-
-(*-----------------------------------------------------------------------*)
-subsection {* VDM while statement in Isabelle *}
+subsection \<open> VDM while statement in Isabelle \<close>
 
 (*
-text {*
+text \<open>
   While and for loops are imperative statements that are tricky to implement in Isabelle. 
   A simple alternative (in most cases) version uses tail-recursive functions.
 
@@ -2239,14 +2338,14 @@ text {*
 
   Functions and pattern matching with records can be tricky. Instead, I will unpack the record
   as parameters. A version with the packaged state can be easily created on top.
-*}
+\<close>
 
 fun naive_play_game0 :: "Move \<Rightarrow> Player \<Rightarrow> Moves \<Rightarrow> NimSt"
 where
   "naive_play_game0 l p []   = \<lparr> limit = l, current = p, moves = [] \<rparr>"
 | "naive_play_game0 l p (x#xs) = (naive_play_game0 l p xs)"
 *) (*<*) thm while_def (*>*)
-text {* 
+text \<open> 
   The VDM while statement
 
 \begin{vdmsl}[breaklines=true]
@@ -2279,12 +2378,12 @@ text {*
   as well as auxiliary functions and operations pre/post conditions are enforced, we create
   auxiliary Isabelle definitions to enable us to call the appropriate pre/post at the right 
   place. Moreover, loops should contain an invariant and variant statement (\textbf{TODO}!).
-*}
+\<close>
 
 (*-----------------------------------------------------------------------*)
-subsection {* @{term naive_play_game} operation *}
+subsection \<open> @{term naive_play_game} operation \<close>
 
-text{*
+text\<open>
 \begin{vdmsl}[breaklines=true]
 naive_play_game() ==
 	((while moves_left(moves) > 0 do
@@ -2296,10 +2395,10 @@ ext wr current, moves
 pre moves_left(moves) = MAX_PILE
 post moves_left(moves) = 0;
 \end{vdmsl}
-*}
+\<close>
 
 (*+++++++++++++++++++++++++++++++++++++++++++++++++++++++++++++++++++++++*)
-subsubsection {* Specification *}
+subsubsection \<open> Specification \<close>
 
 definition
   pre_naive_play_game :: "NimSt \<Rightarrow> \<bool>"
@@ -2315,16 +2414,12 @@ definition
   post_naive_play_game :: "NimSt \<Rightarrow> NimSt \<Rightarrow> \<bool>"
 where
   "post_naive_play_game bst ast \<equiv> 
-      inv_Nim bst \<and> inv_Nim ast \<and>
-      (let ams = (moves ast) in
-        pre_moves_left ams \<and> 
-        post_moves_left ams (moves_left ams) \<and>
-        moves_left ams = 0)"
-
-
+      pre_naive_play_game bst \<longrightarrow>  
+      inv_Nim ast \<and>
+      (let ams = (moves ast) in moves_left ams = 0)"
 
 (*+++++++++++++++++++++++++++++++++++++++++++++++++++++++++++++++++++++++*)
-subsubsection {* Implementation *}
+subsubsection \<open> Implementation \<close>
 
 definition 
   naive_play_game_inner_play :: "NimSt \<Rightarrow> NimSt"
@@ -2332,6 +2427,7 @@ where
   "naive_play_game_inner_play bst \<equiv> 
      save (naive_choose_move bst) bst"
 
+term while
 definition
   naive_play_game_loop :: "NimSt \<Rightarrow> NimSt"
 where
@@ -2341,10 +2437,16 @@ where
             bst"
 
 definition
+  naive_play_game0 :: "NimSt \<Rightarrow> NimSt"
+where
+  "naive_play_game0 bst \<equiv> 
+      tally(naive_play_game_loop bst)"
+
+definition
   naive_play_game :: "NimSt \<Rightarrow> NimSt"
 where
   "naive_play_game bst \<equiv> 
-      tally (naive_play_game_loop bst)"
+      (naive_play_game_loop ;; tally, bst)" 
 
 (*<*)
 (* TODO: loop invariant? / post *)
@@ -2361,9 +2463,9 @@ where
 (*>*)
 
 (*-----------------------------------------------------------------------*)
-subsection {* @{term fixed_play_game} operation *}
+subsection \<open> @{term fixed_play_game} operation \<close>
 
-text{*
+text\<open>
 \begin{vdmsl}[breaklines=true]
 fixed_play_game() ==
 	((while moves_left(moves) > 0 do
@@ -2375,25 +2477,23 @@ ext wr current, moves
 pre moves_left(moves) = MAX_PILE
 post moves_left(moves) = 0;
 \end{vdmsl}
-*}
+\<close>
 
 (*+++++++++++++++++++++++++++++++++++++++++++++++++++++++++++++++++++++++*)
-subsubsection {* Specification *}
-
-text {* TODO *}
+subsubsection \<open> Specification \<close>
 
 definition
   pre_fixed_play_game :: "NimSt \<Rightarrow> \<bool>"
 where
-  "pre_fixed_play_game bst \<equiv>  True"
+  "pre_fixed_play_game bst \<equiv> pre_naive_play_game bst"
 
 definition
   post_fixed_play_game :: "NimSt \<Rightarrow> NimSt \<Rightarrow> \<bool>"
 where
-  "post_fixed_play_game bst ast \<equiv> True"
+  "post_fixed_play_game bst ast \<equiv> post_naive_play_game bst ast"
 
 (*+++++++++++++++++++++++++++++++++++++++++++++++++++++++++++++++++++++++*)
-subsubsection {* Implementation *}
+subsubsection \<open> Implementation \<close>
 
 definition
   fixed_play_game_loop :: "NimSt \<Rightarrow> NimSt"
@@ -2406,12 +2506,12 @@ where
 definition
   fixed_play_game :: "NimSt \<Rightarrow> NimSt"
 where
-  "fixed_play_game bst \<equiv> tally (fixed_play_game_loop bst)"
+  "fixed_play_game bst \<equiv> (naive_play_game_loop ;; tally, bst)"
 
 (*-----------------------------------------------------------------------*)
-subsection {* @{term first_win_game} operation *}
+subsection \<open> @{term first_win_game} operation \<close>
 
-text{*
+text\<open>
 \begin{vdmsl}[breaklines=true]
 first_win_game() ==
 	((while moves_left(moves) > 0 do
@@ -2428,12 +2528,10 @@ ext wr current, moves
 pre moves_left(moves) = MAX_PILE
 post moves_left(moves) = 0;
 \end{vdmsl}
-*}
+\<close>
 
 (*+++++++++++++++++++++++++++++++++++++++++++++++++++++++++++++++++++++++*)
-subsubsection {* Specification *}
-
-text {* TODO? *}
+subsubsection \<open> Specification \<close>
 
 definition
   pre_first_win_game :: "NimSt \<Rightarrow> \<bool>"
@@ -2446,7 +2544,7 @@ where
   "post_first_win_game bst ast \<equiv> post_naive_play_game bst ast"
 
 (*+++++++++++++++++++++++++++++++++++++++++++++++++++++++++++++++++++++++*)
-subsubsection {* Implementation *}
+subsubsection \<open> Implementation \<close>
 
 definition
   first_win_game_loop :: "NimSt \<Rightarrow> NimSt"
@@ -2465,13 +2563,12 @@ where
 definition
   first_win_game :: "NimSt \<Rightarrow> NimSt"
 where
-  "first_win_game bst \<equiv> 
-      tally (first_win_game_loop bst)"
+  "first_win_game bst \<equiv> (first_win_game_loop ;; tally, bst)" 
 
 (*************************************************************************)
-section {* VDM proof obligations *}
+section \<open> VDM proof obligations \<close>
 
-text {*
+text \<open>
   The Overture proof obligation generator (POG) can be executed either from the
   context menu of the corresponding project, via the command line, or via the console. 
   The context menu fills in the PO explorer view, whereas the console prints POs in 
@@ -2483,18 +2580,18 @@ text {*
   implicitly enforced/expected type invariants. So just like for other definitions, type invariants
   need to be explicit added for quantified variables. Isabelle on the other hand, will do base type inference.
   For \texttt{NimFull.vdmsl}, POG generated $40$ POs, some of which I discuss below.
-*}
+\<close>
 
 (*-----------------------------------------------------------------------*)
-subsection {* PO1 *}
+subsection \<open> PO1 \<close>
 
-text{*
+text\<open>
 Move: type invariant satisfiable obligation @ in 'NimFull' (./NimFull.vdmsl) at line 23:1
 \begin{vdmsl}[breaklines=true]
 (exists m:Move & (m <= MAX_MOV))
 Proof Obligation 01: (Unproved)
 \end{vdmsl}
-*}
+\<close>
 
 definition 
   PO01_move_type_inv_sat_obl :: \<bool>
@@ -2503,7 +2600,7 @@ where
 
 theorem PO01_move_type_inv_sat_obl
 unfolding PO01_move_type_inv_sat_obl_def inv_Move_def 
-using inv_VDMNat1_def by force --"SH"
+using inv_VDMNat1_def by force (* SH *)
 
 definition 
   PO01_move_type_inv_sat_obl_gen :: \<bool>
@@ -2512,20 +2609,20 @@ where
 
 theorem PO01_move_type_inv_sat_obl_gen
   unfolding PO01_move_type_inv_sat_obl_gen_def  
-using inv_VDMNat1_def n1_MM by blast --"SH"
+using inv_VDMNat1_def n1_MM by blast (* SH *)
 
 (*-----------------------------------------------------------------------*)
-subsection {* PO2 *}
+subsection \<open> PO2 \<close>
 
-text{*
+text\<open>
 \begin{vdmsl}[breaklines=true]
 Moves: legal sequence application obligation @ in 'NimFull' (./NimFull.vdmsl) at line 32:30
 (forall s:seq of (Move) & ((sum_elems(s) <= MAX_PILE) => ((sum_elems(s) = MAX_PILE) => ((len s) in set (inds s)))))
 Proof Obligation 02: (Unproved)
 \end{vdmsl}
-*}
+\<close>
 
-text {*
+text \<open>
   For universally quantified proofs, type invariants are to be considered as a guard. 
   That is, if the invariant hold, then the PO must follow;~otherwise, we do not care. 
   That is an accurate representation for what Isabelle type inference does to the bound 
@@ -2538,7 +2635,7 @@ text {*
   \]
 
   So, whenever @{term "x \<notin> \<nat>"}, then we do not care about the value of the expression.
-*}
+\<close>
 
 value "len [a,b]"
 value "inds [a,b]"
@@ -2550,26 +2647,28 @@ where
       (sum_elems s \<le> MAX_PILE \<longrightarrow> (sum_elems s = MAX_PILE) \<longrightarrow> (len s \<in> inds s))"
 
 theorem PO02_moves_legal_seq_app_obl
-  unfolding PO02_moves_legal_seq_app_obl_def inv_Moves_def VDMSeq_def
+  unfolding PO02_moves_legal_seq_app_obl_def inv_Moves_def
 apply (intro allI impI)
 apply simp
 apply (erule sum_elems.elims)
-apply simp+
+   apply simp+
+  unfolding len_def 
+  apply simp
 done
 
 (*-----------------------------------------------------------------------*)
-subsection {* PO3 *}
+subsection \<open> PO3 \<close>
 
-text{*
+text\<open>
 \begin{vdmsl}[breaklines=true]
 Moves: type invariant satisfiable obligation @ in 'NimFull' (./NimFull.vdmsl) at line 26:1
 (exists s:Moves & ((sum_elems(s) <= MAX_PILE) and ((sum_elems(s) = MAX_PILE) => (s((len s)) = 1))))
 Proof Obligation 03: (Unproved)
 \end{vdmsl}
-*}
+\<close>
 
-text {* For commonly used combinations of definitions to be unfolded, you can use a 
-  @{term lemmas} command to give a synonym for a group of definitions. *}
+text \<open> For commonly used combinations of definitions to be unfolded, you can use a 
+  @{term lemmas} command to give a synonym for a group of definitions. \<close>
   
 definition 
   PO03_moves_type_inv_sat_obl :: \<bool>
@@ -2578,14 +2677,14 @@ where
       (sum_elems s \<le> MAX_PILE \<longrightarrow> (sum_elems s = MAX_PILE) \<longrightarrow> applyVDMSeq s (len s) = 1)"
 
 theorem PO03_moves_type_inv_sat_obl
-  unfolding PO03_moves_type_inv_sat_obl_def  VDMSeq_def  oops 
+  unfolding PO03_moves_type_inv_sat_obl_def applyVDMSeq_def  oops 
 
-text {* Postcondition of @{term sum_elems} is just @{term True}, hence this  *}
+text \<open> Postcondition of @{term sum_elems} is just @{term True}, hence this  \<close>
 
 (*-----------------------------------------------------------------------*)
-subsection {* PO4 *}
+subsection \<open> PO4 \<close>
 
-text{*
+text\<open>
 \begin{vdmsl}[breaklines=true]
 sum_elems: function establishes postcondition obligation @ in 'NimFull' (./NimFull.vdmsl) at line 37:1
 (forall s:seq of (Move) & post_sum_elems(s, (cases s :
@@ -2594,7 +2693,7 @@ sum_elems: function establishes postcondition obligation @ in 'NimFull' (./NimFu
  end)))
 Proof Obligation 04: (Unproved)
 \end{vdmsl}
-*}
+\<close>
 
 definition
   PO04_sum_elems_post_obl :: "\<bool>"
@@ -2610,97 +2709,97 @@ apply (case_tac ms)
 apply (subgoal_tac "inv_SeqElems inv_Move ms")
 apply (frule l_sum_elems_nat)
   apply (simp add: l_sum_elems_nat)
-  apply (simp add: add_pos_nonneg l_inv_SeqElems_Cons l_sum_elems_nat)
+  using l_pre_sum_elems apply force
 nitpick[user_axioms]
 find_theorems "sum_elems _"
 oops
 
-text {* Because @{term sum_elems} is recursively defined in Isabelle,
+text \<open> Because @{term sum_elems} is recursively defined in Isabelle,
   its proof obligations from Overure related to recursive definitions are irrelevant. 
   That is because Isabelle automatically proves such POs implicitly. For example,
   
   @{thm[display] sum_elems.induct sum_elems.cases}
-*}
+\<close>
 
 (*<*)
 find_theorems name:sum_elems
 (*-----------------------------------------------------------------------*)
-subsection {* PO5 *}
+subsection \<open> PO5 \<close>
 
-text{*
+text\<open>
 \begin{vdmsl}[breaklines=true]
 sum_elems: recursive function obligation @ in 'NimFull' (./NimFull.vdmsl) at line 41:17
 (forall s:seq of (Move) & ((not ([] = s)) => (exists [x] ^ xs:seq of (Move) & ((([x] ^ xs) = s) => let [x] ^ xs = s in (sum_elems_measure(s) > sum_elems_measure(xs))))))
 Proof Obligation 05: (Unproved)
 \end{vdmsl}
-*}
+\<close>
 
 (*-----------------------------------------------------------------------*)
-subsection {* PO6 *}
+subsection \<open> PO6 \<close>
 
-text{*
+text\<open>
 \begin{vdmsl}[breaklines=true]
 sum_elems: cases exhaustive obligation @ in 'NimFull' (./NimFull.vdmsl) at line 39:2
 (forall s:seq of (Move) & ((s = []) or (exists [x] ^ xs:seq of (Move) & (s = ([x] ^ xs)))))
 Proof Obligation 06: (Unproved)
 \end{vdmsl}
-*}
+\<close>
 
 (*-----------------------------------------------------------------------*)
-subsection {* PO7 *}
+subsection \<open> PO7 \<close>
 
-text{*
+text\<open>
 \begin{vdmsl}[breaklines=true]
 fair_play: legal function application obligation @ in 'NimFull' (./NimFull.vdmsl) at line 59:25
 (forall p:Player, ms:Moves & pre_who_plays_next(ms))
 Proof Obligation 07: (Unproved)
 \end{vdmsl}
-*}
+\<close>
 (*-----------------------------------------------------------------------*)
-subsection {* PO8 *}
+subsection \<open> PO8 \<close>
 
-text{*
+text\<open>
 \begin{vdmsl}[breaklines=true]
 moves_left: type compatibility obligation @ in 'NimFull' (./NimFull.vdmsl) at line 61:1
 (forall ms:Moves & ((MAX_PILE - sum_elems(ms)) >= 0))
 Proof Obligation 08: (Unproved)
 \end{vdmsl}
-*}
+\<close>
 (*-----------------------------------------------------------------------*)
-subsection {* PO9*}
+subsection \<open> PO9\<close>
 
-text{*
+text\<open>
 \begin{vdmsl}[breaklines=true]
 play_move: function establishes postcondition obligation @ in 'NimFull' (./NimFull.vdmsl) at line 64:1
 (forall p:Player, m:Move, s:Moves & (pre_play_move(p, m, s) => post_play_move(p, m, s, (s ^ [m]))))
 Proof Obligation 09: (Unproved)
 \end{vdmsl}
-*}
+\<close>
 (*-----------------------------------------------------------------------*)
-subsection {* PO10 *}
+subsection \<open> PO10 \<close>
 
-text{*
+text\<open>
 \begin{vdmsl}[breaklines=true]
 play_move: type compatibility obligation @ in 'NimFull' (./NimFull.vdmsl) at line 64:1
 (forall p:Player, m:Move, s:Moves & (((moves_left(s) <> 1) => ((m < moves_left(s)) and ((moves_left(s) > 0) and fair_play(p, s)))) => inv_Moves((s ^ [m]))))
 Proof Obligation 10: (Unproved)
 \end{vdmsl}
-*}
+\<close>
 
 (*-----------------------------------------------------------------------*)
-subsection {* PO11 *}
-text{*
+subsection \<open> PO11 \<close>
+text\<open>
 \begin{vdmsl}[breaklines=true]
 who_won_invariant: legal function application obligation @ in 'NimFull' (./NimFull.vdmsl) at line 93:11
 (forall winner:Player, moves:Moves & ((moves_left(moves) = 0) => pre_who_plays_next(moves)))
 Proof Obligation 11: (Unproved)
 \end{vdmsl}
-*}
+\<close>
 
 (*-----------------------------------------------------------------------*)
-subsection {* P12 *}
+subsection \<open> P12 \<close>
 
-text{*
+text\<open>
 \begin{vdmsl}[breaklines=true]
 first_player: function establishes postcondition obligation @ in 'NimFull' (./NimFull.vdmsl) at line 102:1
 post_first_player((if isFirst(<P1>)
@@ -2708,23 +2807,23 @@ then <P1>
 else <P2>))
 Proof Obligation 12: (Unproved)
 \end{vdmsl}
-*}
+\<close>
 
 (*-----------------------------------------------------------------------*)
-subsection {* P13 *}
+subsection \<open> P13 \<close>
 
-text{*
+text\<open>
 \begin{vdmsl}[breaklines=true]
 first_player_inds: function establishes postcondition obligation @ in 'NimFull' (./NimFull.vdmsl) at line 106:1
 (forall ms:Moves & post_first_player_inds(ms, {i | i in set (inds ms) & ((i mod 2) <> 0)}))
 Proof Obligation 13: (Unproved)
 \end{vdmsl}
-*}
+\<close>
 
 (*-----------------------------------------------------------------------*)
-subsection {* P14 *}
+subsection \<open> P14 \<close>
 
-text{*
+text\<open>
 \begin{vdmsl}[breaklines=true]
 moves_of: legal sequence application obligation @ in 'NimFull' (./NimFull.vdmsl) at line 113:6
 (forall ms:Moves, first:bool & let idxs:set of (nat1) = first_player_inds(ms) in (forall i in set (if first
@@ -2732,34 +2831,34 @@ then idxs
 else ((inds ms) \ idxs)) & (i in set (inds ms))))
 Proof Obligation 14: (Unproved)
 \end{vdmsl}
-*}
+\<close>
 
 (*-----------------------------------------------------------------------*)
-subsection {* P15 *}
+subsection \<open> P15 \<close>
 
-text{*
+text\<open>
 \begin{vdmsl}[breaklines=true]
 best_move: function establishes postcondition obligation @ in 'NimFull' (./NimFull.vdmsl) at line 119:1
 (forall moves:Moves & post_best_move(moves, ((moves_left(moves) - 1) mod (MAX_MOV + 1))))
 Proof Obligation 15: (Unproved)
 \end{vdmsl}
-*}
+\<close>
 
 (*-----------------------------------------------------------------------*)
-subsection {* P16 *}
+subsection \<open> P16 \<close>
 
-text{*
+text\<open>
 \begin{vdmsl}[breaklines=true]
 best_move: type compatibility obligation @ in 'NimFull' (./NimFull.vdmsl) at line 119:1
 (forall moves:Moves & (((moves_left(moves) - 1) mod (MAX_MOV + 1)) >= 0))
 Proof Obligation 16: (Unproved)
 \end{vdmsl}
-*}
+\<close>
 
 (*-----------------------------------------------------------------------*)
-subsection {* P17 *}
+subsection \<open> P17 \<close>
 
-text{*
+text\<open>
 \begin{vdmsl}[breaklines=true]
 flip_current_player: function establishes postcondition obligation @ in 'NimFull' (./NimFull.vdmsl) at line 129:1
 (forall p:Player & post_flip_current_player(p, (if (p = <P1>)
@@ -2767,78 +2866,78 @@ then <P2>
 else <P1>)))
 Proof Obligation 17: (Unproved)
 \end{vdmsl}
-*}
+\<close>
 
 (*-----------------------------------------------------------------------*)
-subsection {* P18 *}
+subsection \<open> P18 \<close>
 
-text{*
+text\<open>
 \begin{vdmsl}[breaklines=true]
 limit, limit~, current, current~, moves, moves~, Nim, Nim~: state invariant satisfiable obligation @ in 'NimFull' (./NimFull.vdmsl) at line 133:7
 (exists limit:Move, current:Player, moves:Moves & ((limit < MAX_PILE) and (fair_play(current, moves) and isFirst(<P1>))))
 Proof Obligation 18: (Unproved)
 \end{vdmsl}
-*}
+\<close>
 
 (*-----------------------------------------------------------------------*)
-subsection {* P19 *}
+subsection \<open> P19 \<close>
 
-text{*
+text\<open>
 \begin{vdmsl}[breaklines=true]
 flip_player: state invariant holds obligation @ in 'NimFull' (./NimFull.vdmsl) at line 170:2
 let mk_Nim(limit, current, moves) = Nim in ((limit < MAX_PILE) and (fair_play(current, moves) and isFirst(<P1>)))
 Proof Obligation 19: (Unproved)
 \end{vdmsl}
-*}
+\<close>
 
 (*-----------------------------------------------------------------------*)
-subsection {* P20 *}
+subsection \<open> P20 \<close>
 
-text{*
+text\<open>
 \begin{vdmsl}[breaklines=true]
 naive_choose_move: let be st existence obligation @ in 'NimFull' (./NimFull.vdmsl) at line 189:6
 (exists m in set {1, ... ,min(MAX_MOV, moves_left(moves))} & true)
 Proof Obligation 20: (Unproved)
 \end{vdmsl}
-*}
+\<close>
 
 (*-----------------------------------------------------------------------*)
-subsection {* P21 *}
+subsection \<open> P21 \<close>
 
-text{*
+text\<open>
 \begin{vdmsl}[breaklines=true]
 naive_choose_move: type compatibility obligation @ in 'NimFull' (./NimFull.vdmsl) at line 187:1
 (inv_Move(r) and is_(r, nat1))
 Proof Obligation 21: (Unproved)
 \end{vdmsl}
-*}
+\<close>
 
 (*-----------------------------------------------------------------------*)
-subsection {* P22 *}
+subsection \<open> P22 \<close>
 
-text{*
+text\<open>
 \begin{vdmsl}[breaklines=true]
 io_choose_move: type compatibility obligation @ in 'NimFull' (./NimFull.vdmsl) at line 196:1
 (inv_Move(r) and is_(r, nat1))
 Proof Obligation 22: (Unproved)
 \end{vdmsl}
-*}
+\<close>
 
 (*-----------------------------------------------------------------------*)
-subsection {* P23 *}
+subsection \<open> P23 \<close>
 
-text{*
+text\<open>
 \begin{vdmsl}[breaklines=true]
 fixed_choose_move: legal function application obligation @ in 'NimFull' (./NimFull.vdmsl) at line 214:10
 ((moves_left(moves) > 0) => ((r < moves_left(moves)) => (will_first_player_win() => pre_who_plays_next(moves))))
 Proof Obligation 23: (Unproved)
 \end{vdmsl}
-*}
+\<close>
 
 (*-----------------------------------------------------------------------*)
-subsection {* P24 *}
+subsection \<open> P24 \<close>
 
-text{*
+text\<open>
 \begin{vdmsl}[breaklines=true]
 fixed_choose_move: legal function application obligation @ in 'NimFull' (./NimFull.vdmsl) at line 215:15
 ((moves_left(moves) > 0) => (((r < moves_left(moves)) and (will_first_player_win() and isFirst(who_plays_next(moves)))) => pre_play_move((if (current = <P1>)
@@ -2846,23 +2945,23 @@ then <P2>
 else <P1>), r, moves)))
 Proof Obligation 24: (Unproved)
 \end{vdmsl}
-*}
+\<close>
 
 (*-----------------------------------------------------------------------*)
-subsection {* P25 *}
+subsection \<open> P25 \<close>
 
-text{*
+text\<open>
 \begin{vdmsl}[breaklines=true]
 fixed_choose_move: legal sequence application obligation @ in 'NimFull' (./NimFull.vdmsl) at line 204:9
 (((len moves) + 1) in set (inds FIXED_PLAY))
 Proof Obligation 25: (Unproved)
 \end{vdmsl}
-*}
+\<close>
 
 (*-----------------------------------------------------------------------*)
-subsection {* P26 *}
+subsection \<open> P26 \<close>
 
-text{*
+text\<open>
 \begin{vdmsl}[breaklines=true]
 first_player_winning_choose_move: legal function application obligation @ in 'NimFull' (./NimFull.vdmsl) at line 228:39
 ((moves_left(moves) > 0) => (((r < moves_left(moves)) and will_first_player_win()) => pre_play_move((if (current = <P1>)
@@ -2870,23 +2969,23 @@ then <P2>
 else <P1>), r, moves)))
 Proof Obligation 26: (Unproved)
 \end{vdmsl}
-*}
+\<close>
 
 (*-----------------------------------------------------------------------*)
-subsection {* P27 *}
+subsection \<open> P27 \<close>
 
-text{*
+text\<open>
 \begin{vdmsl}[breaklines=true]
 first_player_winning_choose_move: type compatibility obligation @ in 'NimFull' (./NimFull.vdmsl) at line 218:1
 (inv_Move(r) and is_(r, nat1))
 Proof Obligation 27: (Unproved)
 \end{vdmsl}
-*}
+\<close>
 
 (*-----------------------------------------------------------------------*)
-subsection {* P28 *}
+subsection \<open> P28 \<close>
 
-text{*
+text\<open>
 \begin{vdmsl}[breaklines=true]
 save, ms: legal function application obligation @ in 'NimFull' (./NimFull.vdmsl) at line 232:22
 pre_play_move((if (current = <P1>)
@@ -2894,34 +2993,34 @@ then <P2>
 else <P1>), choice, moves)
 Proof Obligation 28: (Unproved)
 \end{vdmsl}
-*}
+\<close>
 
 (*-----------------------------------------------------------------------*)
-subsection {* P29 *}
+subsection \<open> P29 \<close>
 
-text{*
+text\<open>
 \begin{vdmsl}[breaklines=true]
 save: state invariant holds obligation @ in 'NimFull' (./NimFull.vdmsl) at line 236:3
 (inv_Nim(mk_Nim(limit, current, moves)) => inv_Nim(mk_Nim(limit, next, ms)))
 Proof Obligation 29: (Unproved)
 \end{vdmsl}
-*}
+\<close>
 
 (*-----------------------------------------------------------------------*)
-subsection {* P30 *}
+subsection \<open> P30 \<close>
 
-text{*
+text\<open>
 \begin{vdmsl}[breaklines=true]
 naive_play_game: while loop termination obligation @ in 'NimFull' (./NimFull.vdmsl) at line 252:4
 ...
 Proof Obligation 30: (Unproved)
 \end{vdmsl}
-*}
+\<close>
 
 (*-----------------------------------------------------------------------*)
-subsection {* P31 *}
+subsection \<open> P31 \<close>
 
-text{*
+text\<open>
 \begin{vdmsl}[breaklines=true]
 naive_play_game: operation call obligation @ in 'NimFull' (./NimFull.vdmsl) at line 253:4
 pre_play_move((if (current = <P1>)
@@ -2929,23 +3028,23 @@ then <P2>
 else <P1>), naive_choose_move(), moves)
 Proof Obligation 31: (Unproved)
 \end{vdmsl}
-*}
+\<close>
 
 (*-----------------------------------------------------------------------*)
-subsection {* P32 *}
+subsection \<open> P32 \<close>
 
-text{*
+text\<open>
 \begin{vdmsl}[breaklines=true]
 fixed_play_game: while loop termination obligation @ in 'NimFull' (./NimFull.vdmsl) at line 262:4
 ...
 Proof Obligation 32: (Unproved)
 \end{vdmsl}
-*}
+\<close>
 
 (*-----------------------------------------------------------------------*)
-subsection {* P33 *}
+subsection \<open> P33 \<close>
 
-text{*
+text\<open>
 \begin{vdmsl}[breaklines=true]
 fixed_play_game: operation call obligation @ in 'NimFull' (./NimFull.vdmsl) at line 263:4
 pre_play_move((if (current = <P1>)
@@ -2953,23 +3052,23 @@ then <P2>
 else <P1>), fixed_choose_move(), moves)
 Proof Obligation 33: (Unproved)
 \end{vdmsl}
-*}
+\<close>
 
 (*-----------------------------------------------------------------------*)
-subsection {* P34 *}
+subsection \<open> P34 \<close>
 
-text{*
+text\<open>
 \begin{vdmsl}[breaklines=true]
 first_win_game: while loop termination obligation @ in 'NimFull' (./NimFull.vdmsl) at line 272:4
 ...
 Proof Obligation 34: (Unproved)
 \end{vdmsl}
-*}
+\<close>
 
 (*-----------------------------------------------------------------------*)
-subsection {* P35 *}
+subsection \<open> P35 \<close>
 
-text{*
+text\<open>
 \begin{vdmsl}[breaklines=true]
 first_win_game: operation call obligation @ in 'NimFull' (./NimFull.vdmsl) at line 277:4
 pre_play_move((if (current = <P1>)
@@ -2977,64 +3076,63 @@ then <P2>
 else <P1>), choice, moves)
 Proof Obligation 35: (Unproved)
 \end{vdmsl}
-*}
+\<close>
 
 (*-----------------------------------------------------------------------*)
-subsection {* P36 *}
+subsection \<open> P36 \<close>
 
-text{*
+text\<open>
 \begin{vdmsl}[breaklines=true]
 reset: state invariant holds obligation @ in 'NimFull' (./NimFull.vdmsl) at line 288:3
 (inv_Nim(mk_Nim(limit, current, moves)) => inv_Nim(mk_Nim(limit, first_player(), [])))
 Proof Obligation 36: (Unproved)
 \end{vdmsl}
-*}
+\<close>
 
 (*-----------------------------------------------------------------------*)
-subsection {* P37 *}
+subsection \<open> P37 \<close>
 
-text{*
+text\<open>
 \begin{vdmsl}[breaklines=true]
 all_play_game: operation call obligation @ in 'NimFull' (./NimFull.vdmsl) at line 301:3
 (moves_left(moves) = MAX_PILE)
 Proof Obligation 37: (Unproved)
 \end{vdmsl}
-*}
+\<close>
 
 (*-----------------------------------------------------------------------*)
-subsection {* P38 *}
+subsection \<open> P38 \<close>
 
-text{*
+text\<open>
 \begin{vdmsl}[breaklines=true]
 all_play_game: operation call obligation @ in 'NimFull' (./NimFull.vdmsl) at line 306:3
 ((moves_left(moves) = 0) => (true => (moves_left(moves) = MAX_PILE)))
 Proof Obligation 38: (Unproved)
 \end{vdmsl}
-*}
+\<close>
 
 (*-----------------------------------------------------------------------*)
-subsection {* P39 *}
+subsection \<open> P39 \<close>
 
 
-text{*
+text\<open>
 \begin{vdmsl}[breaklines=true]
 all_play_game: operation call obligation @ in 'NimFull' (./NimFull.vdmsl) at line 311:3
 ((moves_left(moves) = 0) => (true => ((moves_left(moves) = 0) => (true => (moves_left(moves) = MAX_PILE)))))
 Proof Obligation 39: (Unproved)
 \end{vdmsl}
-*}
+\<close>
 
 (*-----------------------------------------------------------------------*)
-subsection {* P40 *}
+subsection \<open> P40 \<close>
 
-text{*
+text\<open>
 \begin{vdmsl}[breaklines=true]
 FIXED_PLAY: type compatibility obligation @ in 'NimFull' (./NimFull.vdmsl) at line 316:21
 (inv_Moves([3, 2, 2, 1, 3, 2, 2, 1, 3, 1]) and (((((((((inv_Move(3) and inv_Move(2)) and inv_Move(2)) and inv_Move(1)) and inv_Move(3)) and inv_Move(2)) and inv_Move(2)) and inv_Move(1)) and inv_Move(3)) and inv_Move(1)))
 Proof Obligation 40: (Unproved)
 \end{vdmsl}
-*}
-
+\<close>
 find_theorems name:play_move  
 end
 (*>*)
